common/JWordList.ec
@@ -3,156 +3,91 @@ require import AllCore List Int IntDiv.
 from Jasmin require import JMemory JWord JUtils.
 
 
-(*from JazzCommon*) require import EclibExtra.
+require import EclibExtra.
+
+(* TODO: cleanup!!! *)
+
 require BitEncoding.
 import BitEncoding.BitChunking.
 require import StdOrder.
 import IntOrder.
 
-
-(* TO JUtils *)
-(* MOVE THIS!!! *)
-lemma map2_nilr ['a, 'b, 'c] (f : 'a -> 'b -> 'c) l:
- map2 f l [] = [].
+lemma chunk0 ['a] n (l: 'a list):
+ size l < n =>
+ chunk n l = [].
 proof.
-rewrite -size_eq0 size_map2 /=; smt(size_ge0).
+move=> Hl; rewrite /chunk divz_small; smt(size_ge0 mkseq0).
 qed.
 
-lemma map2_nill ['a, 'b, 'c] (f : 'a -> 'b -> 'c) l:
- map2 f [] l = [].
+(* chunk1 => chunk_size *)
+lemma chunk_size ['a] r (l: 'a list):
+ 0 < r =>
+ size l = r =>
+ chunk r l = [l].
 proof.
-rewrite -size_eq0 size_map2 /=; smt(size_ge0).
+move=> Hr Hsz; rewrite /chunk Hsz divzz (:r<>0) 1:/# b2i1 /=.
+by rewrite /mkseq -iotaredE /= drop0 -Hsz take_size.
 qed.
 
-(* a more general version *)
-lemma nth_map' ['a 'b] (da: 'a) (f: 'a -> 'b) (l: 'a list) db i:
- f da = db =>
- nth db (map f l) i = f (nth da l i).
+lemma behead_chunk ['a] n (l:'a list):
+ behead (chunk n l) = chunk n (drop n l).
 proof.
-move => Hf.
-case: (0 <= i && i < size l) => C.
- by rewrite (nth_map da) //.
-by rewrite !nth_out; smt(size_map).
+case: (size l < n).
+ move=> ?; rewrite drop_oversize 1:/#.
+ rewrite /chunk behead_mkseq.
+ rewrite divz_small /=; first smt(size_ge0).
+ by rewrite mkseq0_le //= mkseq0.
+case: (0 < n); last first.
+rewrite -!lezNgt => ??.
+ by rewrite drop_le0 // !chunk_le0.
+rewrite -lezNgt => ??.
+rewrite /chunk behead_mkseq /=.
+rewrite size_drop // 1:/# lez_maxr 1:/#.
+have ->: (size l - n) %/ n = size l %/ n - 1.
+ have ->: size l = (size l - n) + 1*n by ring.
+ by rewrite divzMDr /#.
+by apply eq_in_mkseq => x Hx /=; rewrite drop_drop /#.
 qed.
 
-(* TO JWord *)
-lemma W8_bits2w_nil:
- W8.bits2w [] = W8.zero.
-proof. by apply W8.ext_eq => i Hi; rewrite /bits2w initiE //=. qed.
-
-(* slightly more general version of W8.bits2K *)
-lemma W8_bits2wK' l:
- size l <= 8 =>
- W8.w2bits (W8.bits2w l) = l ++ nseq (8 - size l) false.
+lemma drop_chunk n k (l: 'a list):
+ 0 < k =>
+ drop n (chunk k l) = chunk k (drop (k*n) l).
 proof.
-move=> H; apply (eq_from_nth false).
- by rewrite size_w2bits size_cat size_nseq; smt(size_ge0).
-move=> i; rewrite size_w2bits => Hi.
-rewrite get_w2bits get_bits2w 1:// nth_cat.
-case: (i < size l) => C //.
-case: ((i - size l) < (8 - size l)) => C2.
- by rewrite !nth_nseq 1:/# nth_out /#.
-smt(nth_out).
+move=> Hk; elim/natind: n l.
+ by move=> n Hn l; rewrite !drop_le0 /#.
+move=> n Hn IH l; rewrite dropS // IH behead_chunk drop_drop 1,2:/#.
+by congr; congr; ring.
 qed.
 
-lemma W8_bits2w_cat_nseq0 bs n:
- W8.bits2w (bs ++ nseq n false)
- = W8.bits2w bs.
+lemma nth_chunk ['a] k (l: 'a list) i:
+ 0 < k =>
+ 0 <= i =>
+ k*i+k <= size l =>
+ nth [] (chunk k l) i =
+ take k (drop (k*i) l).
+proof. by move=> *; rewrite nth_mkseq // /#. qed.
+
+lemma chunk_take_eq ['a] n (l:'a list):
+ 0 < n =>
+ chunk n l = chunk n (take (size l %/ n * n) l).
 proof.
-apply W8.ext_eq => i Hi.
-rewrite /bits2w !initiE //= nth_cat.
-case: (i < size bs) => C //.
-rewrite !nth_nseq_if nth_out; smt(size_ge0).
+move=> Hn; rewrite /chunk.
+have ->: (size (take (size l %/ n * n) l) %/ n) = (size l %/ n).
+ rewrite size_take'; first smt(size_ge0).
+ by rewrite lez_floor 1:/# /= mulzK 1:/#.
+apply eq_in_mkseq => x Hx /=.
+rewrite -{1}(cat_take_drop (size l %/ n * n)).
+rewrite drop_cat size_take'; first smt(size_ge0).
+rewrite lez_floor 1:/# /= mulzC StdOrder.IntOrder.ltr_pmul2r 1:/#.
+move: (Hx); move=> [? ->] /=.
+have E: n <= size (drop (x * n) (take (size l %/ n * n) l)).
+ rewrite size_drop 1:/# lez_maxr; last first.
+  rewrite size_take' 1:/# lez_floor 1:/# /= -Ring.IntID.mulrBl.
+  by rewrite -{1}mulz1 {1}mulzC StdOrder.IntOrder.ler_pmul2r // -ltzS /#.
+ rewrite size_take' 1:/# lez_floor 1:/# /=.
+ smt(size_ge0).
+by rewrite take_cat' E.
 qed.
-
-lemma W64_bits2w_nil:
- W64.bits2w [] = W64.zero.
-proof. by apply W64.ext_eq => i Hi; rewrite /bits2w initiE //=. qed.
-
-lemma W64_bits2wK' l:
- size l <= 64 =>
- W64.w2bits (W64.bits2w l) = l ++ nseq (64 - size l) false.
-proof.
-move=> H; apply (eq_from_nth false).
- by rewrite size_w2bits size_cat size_nseq; smt(size_ge0).
-move=> i; rewrite size_w2bits => Hi.
-rewrite get_w2bits get_bits2w 1:// nth_cat.
-case: (i < size l) => C //.
-case: ((i - size l) < (64 - size l)) => C2.
- by rewrite !nth_nseq 1:/# nth_out /#.
-smt(nth_out).
-qed.
-
-lemma W64_bits2w_cat_nseq0 bs n:
- W64.bits2w (bs ++ nseq n false)
- = W64.bits2w bs.
-proof.
-apply W64.ext_eq => i Hi.
-rewrite /bits2w !initiE //= nth_cat.
-case: (i < size bs) => C //.
-rewrite !nth_nseq_if nth_out; smt(size_ge0).
-qed.
-
-lemma W8u8_to_listK w: pack8 (W8u8.to_list w) = w.
-proof.
-apply W64.ext_eq => k Hk.
-rewrite -(W8u8.unpack8K w); congr; congr.
-rewrite of_listE unpack8E; apply W8u8.Pack.all_eq_eq.
-by rewrite /all_eq /=.
-qed.
-
-lemma W8u8_to_list_pack8 l: 
- size l <= 8 => W8u8.to_list (W8u8.pack8 l) = l ++ nseq (8-size l) W8.zero.
-proof.
-move=> Hl; apply (eq_from_nth W8.zero).
- by rewrite /= size_cat size_nseq /#.
-move => i Hi; rewrite /= in Hi.
-have: (i \in iotared 0 8) by smt().
-move: {Hi} i; rewrite -allP /=.
-rewrite !W8u8.pack8bE // !get_of_list //.
-by rewrite !nth_cat; smt(nth_nseq nth_out).
-qed.
-
-lemma W8u8_pack8_nil: W8u8.pack8 [] = W64.zero.
-proof.
-apply W64.ext_eq => k Hk.
-by rewrite pack8E initiE //= get_of_list 1:/# /=.
-qed.
-
-
-
-lemma W8u8_to_listE (w: W64.t):
- W8u8.to_list w = W8u8.Pack.to_list (unpack8 w).
-proof.
-by rewrite W8u8.unpack8E W8u8.Pack.to_listE /mkseq -iotaredE /=.
-qed.
-
-lemma W8u8_unpack8_inj: injective W8u8.unpack8.
-proof.
-move=> w1 w2.
-rewrite !unpack8E => E.
-apply W64.ext_eq => k Hk.
-rewrite !get_bits8 1..2://; congr.
-have /= <-:= W8u8.Pack.initiE (fun (i : int) => w1 \bits8 i) (k%/8) _.
- smt().
-by rewrite E W8u8.Pack.initiE /#.
-qed.
-
-lemma W8u8_to_list_inj:
- injective W8u8.to_list.
-proof.
-by move=> w1 w2; rewrite !W8u8_to_listE => /W8u8.Pack.to_list_inj /W8u8_unpack8_inj.
-qed.
-
-(** sets a specific byte of a 64-bit word *)
-op w64_set_u8 (w:W64.t, pos: int, x: W8.t): W64.t =
- pack8_t (unpack8 w).[pos <- x].
-
-op w64_xor_u8 (w: W64.t, pos: int, x: W8.t): W64.t =
- let w8u8 = unpack8 w in pack8_t w8u8.[pos <- w8u8.[pos] `^` x].
-
-(* end JWord*)
-
 
 lemma map_chunkK ['a] (f:'a list -> 'a list) n bs:
  0 < n =>
@@ -168,7 +103,6 @@ rewrite E.
 by rewrite map_id chunkK //.
 qed.
 
-
 op chunkremains ['a] n (bs: 'a list) =
  drop (size bs %/ n * n) bs.
 
@@ -179,6 +113,16 @@ rewrite size_drop. smt(size_ge0).
 rewrite lez_maxr; first smt(size_ge0).
 by rewrite {1}(divz_eq (size bs) n) /#.
 qed.
+
+lemma chunkremains_small ['a] n (l: 'a list):
+ size l < n =>
+ chunkremains n l = l.
+proof.
+move=> H; rewrite /chunkremains divz_small.
+ smt(size_ge0).
+by rewrite drop0.
+qed.
+
 
 (** An "extended" version of [chunkK] *)
 lemma chunkK' ['a] r (bs: 'a list):
@@ -196,6 +140,15 @@ rewrite chunkK //.
 by rewrite cat_take_drop.
 qed.
 
+lemma map_chunkK' ['a] f n (bs: 'a list):
+ 0 < n =>
+ (forall (l : 'a list), size l = n => f l = l) =>
+ flatten (map f (chunk n bs)) = take (size bs %/ n * n) bs.
+proof.
+move=> Hn H; rewrite chunk_take_eq // map_chunkK //.
+by rewrite size_take'; smt(size_ge0).
+qed.
+
 lemma chunk_cat' ['a] (l1 l2: 'a list) r:
  0 < r =>
  chunk r (l1++l2)
@@ -211,22 +164,6 @@ rewrite -{1}(cat_take_drop (size l1 %/ r * r) l1) -catA chunk_cat.
 by rewrite -chunk_take_eq //.
 qed.
 
-lemma chunk0 ['a] n (l: 'a list):
- size l < n =>
- chunk n l = [].
-proof.
-move=> Hl; rewrite /chunk divz_small; smt(size_ge0 mkseq0).
-qed.
-
-lemma chunk1 ['a] r (l: 'a list):
- 0 < r =>
- size l = r =>
- chunk r l = [l].
-proof.
-move=> Hr Hsz; rewrite /chunk Hsz divzz (:r<>0) 1:/# b2i1 /=.
-by rewrite /mkseq -iotaredE /= drop0 -Hsz take_size.
-qed.
-
 (** [chunkpad] used to zero-fill the last chunk *)
 op chunkpad ['a] (d:'a) r (l: 'a list) =
  nseq ((-size l)%%r) d.
@@ -234,6 +171,17 @@ op chunkpad ['a] (d:'a) r (l: 'a list) =
 lemma chunkpad_nil ['a] (d: 'a) r:
  chunkpad d r [] = [].
 proof. by rewrite /chunkpad /= nseq0. qed.
+
+lemma size_chunkpad ['a] (d: 'a) r l:
+ 0 < r =>
+ size (chunkpad d r l) = b2i (! r %| size l) * (r - size l %% r).
+proof.
+move=> Hr.
+case: (r %| size l) => [/dvdzE|] C.
+ by rewrite /chunkpad /size_cat size_nseq ler_maxr 1:/# b2i0 -modzNm C.
+rewrite size_nseq ler_maxr ?b2i1 /=; first smt(size_ge0).
+by rewrite -modzNm -modzDl modz_small /#.
+qed.
 
 lemma chunkpadE ['a] (d: 'a) r l:
  0 < r => 
@@ -245,15 +193,6 @@ case: (r %| size l) => [/dvdzE|] C.
 by rewrite /chunkpad /= -modzNm -modzDl modz_small /#.
 qed.
 
-lemma size_chunkpad ['a] (d: 'a) r l:
- 0 < r =>
- size (chunkpad d r l) = b2i (! r %| size l) * (r - size l %% r).
-proof.
-move=> Hr.
-case: (r %| size l) => [/dvdzE|] C.
- by rewrite /chunkpad /size_cat size_nseq ler_maxr 1:/# b2i0 -modzNm C.
-by rewrite b2i1 chunkpadE // C /= size_nseq /#.
-qed.
 
 (** [chunkfill] zero-fills the last chunk *)
 op chunkfill ['a] (d: 'a) r l =
@@ -310,7 +249,7 @@ rewrite b2i1 mkseqS; first smt(size_ge0).
 rewrite cats1; congr => //=.
 rewrite /chunkremains take_oversize.
  by rewrite size_drop; smt(size_ge0).
-by rewrite mulrC.
+smt().
 qed.
 
 lemma chunkify_chunk ['a] n (bs: 'a list):
@@ -353,7 +292,7 @@ move => n_gt0 Hsz0.
  rewrite -{1}(cat_take_drop n l).
 case: (size l < n) => Hsz.
  by rewrite !drop_oversize 1:/# cats0 take_oversize 1:/# chunkify_nil chunkifyE // chunk0 /#.
-rewrite chunkify_cat ?size_take 1..3:/# chunkify_chunk // ?size_take' 1..2:/# chunk1 1:/#. 
+rewrite chunkify_cat ?size_take 1..3:/# chunkify_chunk // ?size_take' 1..2:/# chunk_size 1:/#. 
  by rewrite size_take' /#.
 smt().
 qed.
@@ -414,6 +353,16 @@ rewrite drop0 (:! n * (k + 1) <= 0) 1:/# /= IH ifF 1:/# drop_drop 1..2:/#.
 by congr; congr; ring.
 qed.
 
+lemma divz_minus1 m d:
+ 0 < d => 0 <= m => ! d %| m => (m-1) %/ d = m %/ d.
+proof.
+move=> Hd Hm Hdvd.
+rewrite {1}(divz_eq m d) -addzA divzMDl 1:/#; ring.
+rewrite divz_small //; apply JUtils.bound_abs; split.
+ by move: Hdvd; rewrite dvdzE; smt(JUtils.modz_cmp).
+by move=> ?; smt(JUtils.modz_cmp).
+qed.
+
 (** an alternative definition (normally not as usefull) for
  the size of chunkify *)
 lemma sizechunkifyE n bslen:
@@ -453,34 +402,239 @@ op chunkify_fillsuffix ['a] (d:'a) n sz =
  nseq (b2i (! n %| sz) * (n - sz %% n)) d.
 *)
 
+
+(*
+lemma chunk_truncsize ['a] r (bs: 'a list):
+ 0 < r =>
+ chunk r bs = chunk r (take (size bs %/ r * r) bs).
+proof.
+move=> Hr; rewrite /chunk size_take'; first smt(size_ge0).
+rewrite ifT; first smt(size_ge0). 
+rewrite mulzK 1:/#; apply eq_in_mkseq => i Hi /=.
+rewrite drop_take 1:/# take_take; congr.
+by rewrite lez_minl /#.
+qed.
+*)
+
+lemma chunkpad_drop ['a] d r n (l: 'a list):
+ 0 < r =>
+ 0 <= n*r < size l =>
+ chunkpad d r (drop (n*r) l) = chunkpad d r l.
+proof.
+move=> Hr Hn; rewrite !chunkpadE //.
+ rewrite size_drop 1:/# lez_maxr 1:/#.
+case: (r %| size l) => C.
+ rewrite ifT //.
+ by apply dvdzB => /#.
+rewrite ifF //.
+move: C; apply contra => H.
+ by rewrite (:size l = size l - n*r + n*r) 1:/# dvdzD /#.
+congr. 
+by rewrite -modzBm modzMl /= modz_mod.
+qed.
+
 lemma map_chunkifyK ['a] d (f:'a list -> 'a list) n bs:
  0 < n =>
- (forall l, size l<=n => f l = chunkfill d n l) =>
+ (forall l, 0 < size l <= n => f l = chunkfill d n l) =>
  flatten (map f (chunkify n bs))
- = chunkfill d n bs. (* bs ++ chunkify_fillsuffix d n (size bs).*)
+ = chunkfill d n bs.
 proof.
 move => Hn Hf; rewrite chunkifyE // chunkfillE // map_cat flatten_cat.
 case: (n %| size bs) => C /=.
  rewrite flatten_nil cats0.
  apply map_chunkK => //.
  by move=> l Hl; rewrite Hf 1:/# chunkfillE // Hl dvdzz.
-admitted (*
-rewrite chunkpadE // C /=. (* b2i1 /= chunk_take_eq //.*)
-rewrite -{3}(cat_take_drop (size bs %/ n * n)) -catA; congr.
- rewrite map_chunkK => //.
-  rewrite size_take; first smt(size_ge0).
-  rewrite {2}(divz_eq (size bs) n).
-  case: (size bs %% n = 0)=> ?; first smt().
-  rewrite ifT 1:/#.
-  by rewrite dvdz_mull /#.
- by move=> l Hl; rewrite Hf 1:/# take_size_cat.
-rewrite /flatten /= cats0 Hf; first smt(size_chunkremains).
-rewrite take_cat ifF; first smt(size_chunkremains).
-congr; first smt().
-rewrite take_nseq size_chunkremains ler_minl; smt(size_ge0).
+rewrite map_chunkK' //.
+ by move=> l Hl; rewrite Hf 1:/# chunkfillE // ifT 1:/#.
+rewrite flatten_seq1 Hf.
+ by rewrite size_chunkremains /#.
+rewrite /chunkfill catA /chunkremains cat_take_drop; congr.
+rewrite chunkpad_drop //; smt(size_ge0).
 qed.
-*).
 
+(*
+op chunkfillsize (n sz:int) = (-sz)%%n.
+
+lemma chunkfillsize_cmp n sz:
+ 0 < n => 0 <= chunkfillsize n sz < n.
+proof. move=> Hn; rewrite /chunkfillsize; smt(JUtils.modz_cmp). qed.
+
+lemma chunkfillsizeP n sz k:
+ 0 < n => chunkfillsize n (n*k+sz) = chunkfillsize n sz.
+proof.
+move=> Hn; rewrite /chunkfillsize.
+by rewrite -modzNm mulzC modzMDl modzNm.
+qed.
+
+lemma chunkfillsizeE' n sz:
+ 0 < n => 0 < sz => chunkfillsize n sz = n - 1 - (sz-1) %% n
+by move=> ??; rewrite /chunkfillsize modNz.
+
+lemma chunkfillsizeE n sz:
+ 0 < n => 0 <= sz => chunkfillsize n sz = if n %| sz then 0 else n - sz%%n.
+proof.
+move=> Hn Hsz'.
+case: (n %| sz) .
+ rewrite /chunkfillsize dvdzE -modzNm => ->; smt().
+move=> ?.
+have Hsz : 0 < sz by smt(dvdz0).
+rewrite chunkfillsizeE' //. 
+have ->: n - 1 - (sz - 1) %% n = n - (1 + (sz - 1) %% n) by ring.
+congr; congr.
+by rewrite !modzE divz_minus1 //; ring.
+qed.
+
+op chunkfill ['a] (d:'a) n l = l ++ nseq (chunkfillsize n (size l)) d.
+
+lemma chunkfill_nil ['a] (d:'a) n:
+ chunkfill d n [] = [].
+proof. by rewrite /chunkfill /chunkfillsize nseq0. qed.
+
+hint simplify chunkfill_nil.
+
+lemma dvd_chunkfill ['a] (d:'a) n l:
+ 0 < n => n %| size l => chunkfill d n l = l.
+proof.
+by move=> Hn Hsz; rewrite /chunkfill chunkfillsizeE // ?size_ge0 !Hsz /= nseq0 cats0.
+qed.
+
+lemma size_chunkfill ['a] (d:'a) n l:
+ 0 < n =>
+ size (chunkfill d n l) = (size l - 1) %/ n * n + n.
+proof.
+move=> Hn; rewrite /chunkfill size_cat size_nseq lez_maxr //.
+ smt(chunkfillsize_cmp).
+case: (size l = 0) => E.
+ by rewrite !E /= /chunkfillsize /= divNz //=; ring.
+rewrite chunkfillsizeE' //; first smt(size_ge0).
+have ->: size l + (n - 1 - (size l - 1) %% n) = (size l-1) + n - (size l-1) %% n
+ by ring.
+by rewrite {1}(divz_eq (size l - 1) n); ring.
+qed.
+
+lemma chunkfillP ['a] (d:'a) n l:
+ 0 < n =>
+ n %| size (chunkfill d n l).
+proof.
+move=> Hn; rewrite size_chunkfill //.
+rewrite (: (size l - 1) %/ n * n + n = ((size l - 1) %/ n + 1) * n) 1:/#.
+by rewrite dvdzE modzMl.
+qed.
+
+lemma chunkfillK ['a] (d:'a) n l:
+ 0 < n =>
+ chunkfill d n (chunkfill d n l) = chunkfill d n l.
+proof.
+move=> Hn; rewrite {1}/chunkfill chunkfillsizeE // ?size_ge0.
+by rewrite !chunkfillP //= nseq0 cats0.
+qed.
+
+lemma chunkfill_cat (d:'a) n l1 l2:
+ 0 < n => n %| size l1 => chunkfill d n (l1++l2) = l1 ++ chunkfill d n l2.
+proof.
+move=> H0 Hsz; rewrite /chunkfill -!catA; congr; congr; congr.
+move: Hsz; rewrite size_cat dvdzP => [[k]].
+rewrite mulzC => ->.
+by rewrite chunkfillsizeP.
+qed.
+
+lemma chunkfillK' l (d:'a) n:
+ 0 < n => n %| size l => chunkfill d n l = l.
+proof.
+rewrite /chunkfill => Hn Hsz.
+move: (Hsz); rewrite dvdzP => [[k E]].
+by rewrite chunkfillsizeE // ifT 1:/# nseq0 cats0.
+qed.
+
+lemma chunkfillsize_ge0 k n: 0 < k => 0 <= chunkfillsize k n.
+proof.  by rewrite /chunkfillsize /#. qed.
+
+lemma drop_chunkfill n (d:'a) k l:
+ 0 < k => 0 <= n =>
+ drop (k*n) (chunkfill d k l) = chunkfill d k (drop (k*n) (chunkfill d k l)).
+proof.
+move=> Hk Hn; have := chunkfillP d k l Hk.
+rewrite /chunkfill size_cat size_nseq lez_maxr; first smt(chunkfillsize_ge0).
+move=> Hdvd; pose S:= chunkfillsize _ (size (drop _ _)).
+have ->: S = 0; last by rewrite nseq0 cats0.
+rewrite /S -(chunkfillsizeP _ _ n) // size_drop 1:/# addzC /max size_cat size_nseq. 
+rewrite lez_maxr; first by apply chunkfillsize_ge0.
+case: (0 < size l + chunkfillsize k (size l) - k * n) => E.
+ rewrite Ring.IntID.subrK chunkfillsizeE; first 2 smt(size_ge0 chunkfillsize_ge0).
+ by rewrite !Hdvd.
+by rewrite addzC chunkfillsizeP.
+qed.
+
+lemma nth_chunkfill k (d:'a) n l:
+ 0 < n => nth d (chunkfill d n l) k = nth d l k.
+proof.
+move=> Hn; rewrite /chunkfill nth_cat.
+case: (k < size l) => E //.
+case: (0 <= k - size l < chunkfillsize n (size l)) => ?.
+ by rewrite nth_nseq // nth_out /#.
+rewrite nth_out.
+ by rewrite size_nseq lez_maxr // chunkfillsize_ge0. 
+by rewrite nth_out /#.
+qed.
+
+lemma size_chunkfilled (d:'a) k l:
+ 0 < k =>
+ size (BitEncoding.BitChunking.chunk k (chunkfill d k l))
+ = (size l - 1) %/ k + 1.
+proof.
+move=> Hk; rewrite BitEncoding.BitChunking.size_chunk //.
+by rewrite size_chunkfill // divzMDl 1:/# divzz (:k<>0) 1:/#.
+qed.
+
+lemma head_chunkfilled (d:'a) k l:
+ head [] (BitEncoding.BitChunking.chunk k (chunkfill d k l))
+ = take k (chunkfill d k l).
+proof.
+case: (0 < k) => Hk; last first.
+ by rewrite take_le0 1:/# BitEncoding.BitChunking.chunk_le0 1:/#.
+case: (0 < size l) => Hsz; last first.
+ have ->: l=[] by smt(size_ge0).
+ by rewrite chunkfill_nil /= /BitEncoding.BitChunking.chunk /= mkseq0.
+rewrite -nth0 /BitEncoding.BitChunking.chunk nth_mkseq /=.
+ by rewrite size_chunkfill // /#.
+by rewrite drop0.
+qed.
+
+lemma nth_chunkfilled (d:'a) k l (i:int):
+ 0 < k =>
+ 0 <= i < (size l - 1) %/ k + 1 =>
+ nth [] (BitEncoding.BitChunking.chunk k (chunkfill d k l)) i
+ = take k (drop (k*i) (chunkfill d k l)).
+proof.
+move=> Hk Hi.
+rewrite {1}(:i = i+0) // -nth_drop 1,2:/# drop_chunk // nth0.
+by rewrite drop_chunkfill // 1:/# head_chunkfilled.
+qed.
+
+lemma nth_chunkfilled' dl (d:'a) k l (i:int):
+ 0 < k =>
+ 0 <= i < (size l - 1) %/ k + 1 =>
+ nth dl (BitEncoding.BitChunking.chunk k (chunkfill d k l)) i
+ = mkseq (fun j => nth d l (k*i+j)) k.
+proof.
+move=> Hk Hi.
+rewrite -(nth_inside []); first by rewrite size_chunkfilled.
+rewrite (nth_chunkfilled d k l i) //.
+have Hsz: size (take k (drop (k * i) (chunkfill d k l))) = k.
+ rewrite size_take' 1:/# size_drop 1:/# size_chunkfill //.
+ rewrite lez_maxr; first smt(size_ge0).
+ have: k <= (size l - 1) %/ k * k + k - k * i.
+  by move: Hi => [?]; rewrite ltzE => [?] /#.
+ smt().
+apply (eq_from_nth d); first by rewrite Hsz size_mkseq /#.
+rewrite Hsz => j Hj.
+rewrite nth_take 1,2:/# nth_drop 1,2:/# nth_chunkfill 1:/#.
+by rewrite nth_mkseq.
+qed.
+*)
+
+
+(* END-MOVE THIS??? *)
 
 abstract theory ListEmbedding.
 
@@ -524,12 +678,17 @@ proof. by elim: l1 => //= x xs IH; rewrite !SSSs_to_TTTs_cons IH catA. qed.
 lemma size_SSSs_to_TTTs l:
  size (SSSs_to_TTTs l) = n*size l.
 proof.
-rewrite /SSSs_to_TTTs size_flatten -map_comp /(\o) /=.
-rewrite StdBigop.Bigint.sumzE.
-rewrite StdBigop.Bigint.BIA.big_mapT /(\o) /=.
-rewrite -(StdBigop.Bigint.BIA.eq_bigr _ (fun (x:SSS) => n)).
- by move=> i /= _; rewrite size_SSS_to_TTTs.
-by rewrite StdBigop.Bigint.big_constz count_predT_eq.
+rewrite /SSSs_to_TTTs (size_flatten' n).
+ by move=> x /mapP [Hx ->]; rewrite size_SSS_to_TTTs.
+by rewrite size_map.
+qed.
+
+lemma SSSs_to_TTTs_flatten ll:
+ SSSs_to_TTTs (flatten ll)
+ = flatten (map SSSs_to_TTTs ll).
+proof.
+elim ll => //= x xs IH.
+by rewrite !flatten_cons SSSs_to_TTTs_cat IH.
 qed.
 
 lemma SSSs_to_TTTs_inj: injective SSSs_to_TTTs.
@@ -556,18 +715,54 @@ rewrite SSS_to_TTTs_nil SSS_from_TTTsK ?size_nseq 1:/# ler_maxr 1:/#.
 by rewrite cat_nseq /#.
 qed.
 
+lemma SSSs_from_TTTs_nil: SSSs_from_TTTs [] = [].
+proof. by rewrite /SSSs_from_TTTs chunkify_nil. qed.
+
+lemma SSSs_from_TTTs_cat l1 l2:
+ n %| size l1 =>
+ SSSs_from_TTTs (l1++l2)
+ = SSSs_from_TTTs l1 ++ SSSs_from_TTTs l2.
+proof. by move=> Hsz; rewrite /SSSs_from_TTTs chunkify_cat ?n_gt0 // !map_cat. qed.
+
 lemma SSSs_from_TTTs_nseq0 k:
  0 <= k =>
  SSSs_from_TTTs (nseq k dTTT) = nseq (k %/ n + b2i (! n %| k)) dSSS.
 proof.
-admit.
-qed.
-
-lemma chunkfill_SSSs_from_TTTs k z l:
- chunkfill dSSS k (SSSs_from_TTTs (l ++ nseq z dTTT))
- = chunkfill dSSS k (SSSs_from_TTTs l).
-proof.
-admit.
+have n_gt0:= n_gt0.
+move=> Hk.
+have L: forall k',
+ 0 <= k' => n %| k' =>
+ SSSs_from_TTTs (nseq k' dTTT) = nseq (k' %/ n) dSSS.
+ move=> k' Hk0' Hk'; rewrite -{1}(divzK n k') //.
+ have: (0 <= k' %/ n) by smt().
+ move: (k' %/ n); elim/natind => //=.
+  move=> n' ??; have ->/=: n'=0 by smt().  
+  by rewrite !nseq0 SSSs_from_TTTs_nil.
+ move=> Hn Hn' IH _.
+ rewrite Ring.IntID.mulrSl -cat_nseq 1..2:/#.
+ rewrite SSSs_from_TTTs_cat.
+  by rewrite size_nseq /#.
+ rewrite IH 1:/# -!cat_nseq 1..2:/# nseq1; congr.
+ rewrite /SSSs_from_TTTs chunkifyE 1:/#.
+ rewrite size_nseq ler_maxr 1:/# dvdzz /=.
+ rewrite map_cat /= cats0 chunk_size 1:/#.
+  by rewrite size_nseq /#.
+ by rewrite /= SSS_from_TTTs_nseq0 /#.
+rewrite {1}(divz_eq k n) -cat_nseq 1..2:/#.
+rewrite SSSs_from_TTTs_cat.
+ by rewrite size_nseq /#.
+rewrite -cat_nseq 1..2:/# L 1..2:/#; congr.
+ smt().
+rewrite dvdzE.
+case: (k %% n = 0) => C/=.
+ by rewrite C b2i0 !nseq0 SSSs_from_TTTs_nil.
+rewrite b2i1 nseq1.
+rewrite /SSSs_from_TTTs chunkifyE 1:/#.
+rewrite size_nseq ler_maxr 1:/# chunk0 /=.
+ by rewrite size_nseq /#.
+rewrite ifF 1:/# /= chunkremains_small.
+ by rewrite size_nseq /#.
+by rewrite SSS_from_TTTs_nseq0 /#.
 qed.
 
 lemma SSSs_to_TTTs_take k l:
@@ -600,6 +795,17 @@ have ->/=: ! (n * (k + 1) < size (SSS_to_TTTs x)).
 by rewrite mulzDr /= IH size_SSS_to_TTTs /#.
 qed.
 
+lemma chunk_SSSs_to_TTTs r l:
+ chunk (n*r) (SSSs_to_TTTs l)
+ = map SSSs_to_TTTs (chunk r l).
+proof.
+have n_gt0:= n_gt0.
+rewrite /chunk map_mkseq /(\o) /=.
+rewrite size_SSSs_to_TTTs divzMpl 1:/#.
+apply eq_mkseq => x /=.
+by rewrite SSSs_to_TTTs_take SSSs_to_TTTs_drop /#.
+qed.
+
 lemma SSSs_to_TTTs_map2 fS' fT' l1 l2:
  (forall x1 x2, SSS_to_TTTs (fS' x1 x2)
  = map2 fT' (SSS_to_TTTs x1) (SSS_to_TTTs x2)) =>
@@ -618,14 +824,6 @@ rewrite IH1; congr.
 by apply Hfg.
 qed.
 
-lemma SSSs_from_TTTs_nil: SSSs_from_TTTs [] = [].
-proof. by rewrite /SSSs_from_TTTs chunkify_nil. qed.
-
-lemma SSSs_from_TTTs_cat l1 l2:
- n %| size l1 =>
- SSSs_from_TTTs (l1++l2)
- = SSSs_from_TTTs l1 ++ SSSs_from_TTTs l2.
-proof. by move=> Hsz; rewrite /SSSs_from_TTTs chunkify_cat ?n_gt0 // !map_cat. qed.
 
 lemma SSSs_from_TTTs_cons l:
  0 < size l =>
@@ -649,12 +847,14 @@ lemma SSSs_from_TTTsK l:
 proof.
 rewrite /SSSs_to_TTTs /SSSs_from_TTTs -map_comp.
 apply map_chunkifyK; first exact n_gt0.
-move=> xs Hxs; rewrite /(\o) SSS_from_TTTsK //.
-admitted (*
-rewrite take_cat ifF 1:/# take_nseq.
-smt(size_ge0).
+move=> xs [Hxs0 Hxsn]; rewrite /(\o) SSS_from_TTTsK //.
+rewrite /chunkfill; congr.
+rewrite chunkpadE ?n_gt0 //.
+case: (n %| size xs) => C.
+ have ->: size xs = n by smt().
+ by rewrite /= nseq0.
+by congr; smt().
 qed.
-*).
 
 lemma SSSs_from_TTTsK_dvd l:
  n %| size l => SSSs_to_TTTs (SSSs_from_TTTs l) = l.
@@ -678,7 +878,7 @@ proof.
 elim/natind: k => /=.
  by move=> k Hk1; rewrite !nseq0_le //; smt(n_gt0).
 move=> k Hk IH; rewrite nseqS // SSSs_to_TTTs_cons IH //.
-rewrite addzC mulzDr mulz1 nseq_add //; first 2 smt(n_gt0).
+rewrite addzC mulzDr mulz1 -cat_nseq //; first 2 smt(n_gt0).
 by rewrite SSS_to_TTTs_nil.
 qed.
 
@@ -725,6 +925,38 @@ by congr; rewrite nth_chunkify //.
 qed.
 
 (*
+lemma chunkfill_SSSs_from_TTTs k l:
+ 0 < k =>
+ SSSs_to_TTTs (chunkfill dSSS k (SSSs_from_TTTs l))
+ = chunkfill dTTT (n*k) l.
+proof.
+have n_gt0:= n_gt0; move=> Hk.
+rewrite /chunkfill SSSs_to_TTTs_cat SSSs_from_TTTsK /chunkfill -catA; congr.
+rewrite !chunkpadE 1..3:/#.
+rewrite size_SSSs_from_TTTs.
+case: (n * k %| size l) => C1.
+ have C1': n %| (n*k) by smt(dvdz_mulr dvdzz).
+ have E: (n %| size l) by smt(dvdz_trans).
+ rewrite !E !b2i0 /=.
+ rewrite ifT.
+  move: C1 => /dvdzP [x ->].
+  rewrite (mulzC n) -mulzA mulzK 1:/# dvdz_mull dvdzz.
+ by rewrite SSSs_to_TTTs_nil.
+case: (n %| size l) => C2.
+ rewrite b2i0 /= ifF.
+  admit.
+ rewrite SSSs_to_TTTs_nseq0; congr.
+ have ->: size l %% (n*k) = n*((size l%/ n) %% k).
+  by rewrite mulz_modr /#.
+ smt().
+rewrite b2i1.
+case: (k %| (size l %/ n + 1)) => C3.
+ rewrite SSSs_to_TTTs_nil cats0; congr.
+ admit.
+rewrite SSSs_to_TTTs_nseq0 cat_nseq 1..2:/#; congr.
+admit.
+qed.
+
 lemma chunkify_SSSs_from_TTTs k l:
  chunkify k (SSSs_from_TTTs l)
  = map SSSs_from_TTTs (chunkify (k*n) l).
@@ -758,7 +990,10 @@ qed.
 
 end ListEmbedding.
 
-
+type bit = bool.
+type bits = bool list.
+type byte = W8.t.
+type bytes = W8.t list.
 
 clone export ListEmbedding as Bytes2Bits
  with
@@ -857,43 +1092,53 @@ move=> x xs IH.
 by rewrite /w64L_to_bytes map_cons flatten_cons w64L_to_bits_cons -IH bytes_to_bits_cat  w64_to_bytes_to_bits //. 
 qed.
 
-(*
-print map_comp.
-print chunkify.
-search mkseq.
-
-lemma bits2bytes2w64s l:
- w64L_from_bytes (bits2bytes l)
- = w64L_from_bits l.
-admitted.
-
-map w64_from_bytes (chunkify 8 (bits2bytes l))
-= map (w64_from_bytes \o bits2bytes) (chunkify 64 l)
-= map w64_from_bytes (map bits2bytes (chunkify 64 l))
-
-ou seja:
-chunkify k (bits2bytes l)
-= map bits2bytes (chunkify (k*8) l)
-
-mkseq (fun i => mkseq (fun k => ) sl)
-= mkseq (
-*)
-
-(*
-lemma nosmt size_ind ['a] (P : 'a list -> bool):
- (forall xs, (forall l, size l < size xs => P l) => P xs) => forall l, P l.
+lemma w64L_from_bytes_from_bits l:
+ w64L_from_bytes (bytes_from_bits l) = w64L_from_bits l.
 proof.
-move=> H.
-have Hind: forall (xs l:'a list), size l <= size xs => P l.
- elim => //=.
-  smt.
- move=> xs Hxs l Hl.
- apply H => *. smt.
-by move=> l; apply (Hind l).
+apply w64L_to_bits_inj.
+rewrite -w64L_to_bytes_to_bits w64L_from_bytesK w64L_from_bitsK.
+rewrite /chunkfill bytes_to_bits_cat bytes_from_bitsK -catA; congr.
+rewrite !chunkpadE // size_bytes_from_bits.
+case: (64 %| size l) => C1.
+ have E: 8 %| size l by smt().
+ rewrite !E !b2i0 /=.
+ by rewrite ifT 1:/# bytes_to_bits_nil.
+case: (8 %| size l) => C2.
+ by rewrite b2i0 /= ifF 1:/# bytes_to_bits_nseq0 /#.
+rewrite b2i1.
+case: (8 %| (size l %/ 8 + 1)) => C3.
+ by rewrite bytes_to_bits_nil cats0 /#.
+by rewrite bytes_to_bits_nseq0 cat_nseq /#.
 qed.
-*)
 
+lemma w64_from_bits_from_bytes l:
+ W64.bits2w (bytes_to_bits l) = pack8 l.
+proof.
+rewrite /bytes_to_bits; apply W64.wordP => i Hi.
+rewrite get_bits2w // (nth_flatten _ 8).
+ by rewrite allP => k /mapP [w [Hw ->]].
+rewrite pack8E initiE //= get_of_list 1:/# -get_w2bits.
+case: (i %/ 8 < size l) => C.
+rewrite (nth_map W8.zero) 1..2:/#.
+have ->: nth [] (map W8.w2bits l) (i %/ 8) = [].
+ by rewrite nth_out ?size_map /#.
+rewrite nth_out ?size_map 1:/#.
+have ->: nth W8.zero l (i %/ 8) = W8.zero.
+ by rewrite nth_out /#.
+by rewrite byte_to_bits_nil nth_nseq 1:/#.
+qed.
 
+lemma w64L_from_bits_from_bytes l:
+ w64L_from_bits (bytes_to_bits l) = w64L_from_bytes l.
+proof.
+apply (eq_from_nth W64.zero); rewrite size_w64L_from_bits size_bytes_to_bits.
+ by rewrite size_w64L_from_bytes /#.
+move=> i Hi.
+rewrite nth_w64L_from_bits 1:/#.
+rewrite (:64*i=8*(8*i)) 1:/# -bytes_to_bits_drop (:64=8*8) 1:/#.
+rewrite -bytes_to_bits_take nth_w64L_from_bytes 1:/#.
+by rewrite w64_from_bits_from_bytes.
+qed.
 
 (*
 (*******************************************************************************)
@@ -1660,7 +1905,7 @@ proof. by move=> Hx; rewrite memread_add //= cats1. qed.
 lemma take_memread n mem ptr k:
  0 <= n => 
  take n (memread mem ptr k) = memread mem ptr (min n k).
-proof. by move=> Hn; rewrite /memread take_mkseq. qed.
+proof. move=> Hn; rewrite /memread take_mkseq' //. qed.
 
 lemma loadW8_memread mem in_ inlen i:
  0 <= i < inlen =>
@@ -1691,7 +1936,6 @@ congr; rewrite W8u8.Pack.initiE 1:/# /= /memread /=.
 rewrite of_listE W8u8.Pack.initiE 1:/# /=.
 by rewrite drop_mkseq 1:/# take_mkseq 1:/# /= nth_mkseq /#.
 qed.
-
 
 lemma memread_split off mem a sz:
  0 <= off <= sz =>
