fips202/FIPS202_SHA3.ec
@@ -10,6 +10,7 @@ require import AllCore List Int IntDiv.
 require BitEncoding.
 import BitEncoding.BitChunking.
 
+
 require export FIPS202_Keccakf1600.
 
 
@@ -19,6 +20,72 @@ op st0 : state = Array25.create W64.zero.
 (** State addition (xor) *)
 op addstate = Array25.map2 W64.(`^`) .
 
+(** Section 4 - SPONGE CONSTRUCTION 
+
+from the spec:
+"""
+The construction employs the following three components:
+- An underlying function on fixed-length strings, denoted by f,
+- A parameter called the rate, denoted by r, and
+- A padding rule, denoted by pad.
+...
+
+The function f maps strings of a single, fixed length, denoted by
+b, to strings of the same length. As in Sec. 3, b is called the width
+of f. The SHA-3 functions, specified in Sec. 6 are instances of the
+sponge construction in which the underlying function f is invertible,
+i.e., a permutation, although the sponge construction does not require
+f to be invertible.
+
+The rate r is a positive integer that is strictly less than the width
+b. The capacity, denoted by c, is the positive integer br. Thus, r +
+c = b.
+
+The padding rule, pad, is a function that produces padding, i.e., a
+string with an appropriate length to append to another string. In
+general, given a positive integer x and a non-negative integer m, the
+output pad(x, m) is a string with the property that m + len(pad(x, m))
+is a positive multiple of x. Within the sponge construction, x = r and
+m = len(N), so that the padded input string can be partitioned into a
+sequence of r-bit strings. Algorithm 9 in Sec. 5.1 specifies the
+padding rule for the KECCAK functions and, hence, the SHA-3 functions.
+
+*)
+
+module type SpongeParams = {
+ proc f(s: state): state
+ proc pad(r x: int): bool list
+}.
+
+
+
+module Sponge1600 (P: SpongeParams) = {
+  (** Algorithm 8 *)
+  proc sponge(r: int, m: bool list, d: int): bool list = {
+    var p, pl, n, s, i, z;
+    p <@ P.pad(r, size m);
+    p <- m ++ p;
+    pl <- chunk r p;
+    n <- (size p) %/ r;
+    s <- st0;
+    i <- 0;
+    while (i < n) { (* absorb *)
+      s <- addstate s (bits2state (nth [] pl i));
+      s <@ P.f(s);
+      i <- i + 1;
+    }
+    (* squeeze *)
+    z <- take r (state2bits s);
+    while (size z < d) {
+      s <@ P.f(s);
+      z <- z ++ take r (state2bits s);
+    }
+    return take d z;
+  }
+}.
+
+(** Section 5 - Keccak *)
+
 
 (** Section 5.1 -- Specification of [pad10*1]
     Algorithm 9 *)
@@ -26,34 +93,20 @@ op pad10star1 (x: int) (m: int): bool list =
  true :: rcons (nseq ((-m-2)%%x) false) true.
 
 
+module Keccakf1600_Params = {
+ proc f = Keccakf1600.keccak_f1600 (* Keccak Permutation *)
+ proc pad(r x: int): bool list = { (* multi-rate padding *)
+  return pad10star1 r x;
+ }
+}.
+
 (** Imperative specification for [Keccak-f1600]. *)
 module Keccak1600 = {
-  (** Section 4 - SPONGE CONSTRUCTION
-      Algorithm 8 *)
-  proc sponge1600_pad10star1(r: int, m: bool list, d: int): bool list = {
-    var p, pl, n, s, i, z;
-    p <- m ++ pad10star1 r (size m);
-    pl <- chunk r p;
-    n <- (size p) %/ r;
-    s <- st0;
-    i <- 0;
-    while (i < n) { (* absorb *)
-      s <- addstate s (bits2state (nth [] pl i));
-      s <@ Keccakf1600.keccak_f1600(s);
-      i <- i + 1;
-    }
-    (* squeeze *)
-    z <- take r (state2bits s);
-    while (size z < d) {
-      s <@ Keccakf1600.keccak_f1600(s);
-      z <- z ++ take r (state2bits s);
-    }
-    return take d z;
-  }
+  module Spng = Sponge1600(Keccakf1600_Params)
   (** Section 5.2 - Specification of KECCAK[c] *)
   proc keccak1600(c: int, m: bool list, outlen: int): bool list = {
     var z;
-    z <@ sponge1600_pad10star1(keccak_b - c, m, outlen);
+    z <@ Spng.sponge(keccak_b - c, m, outlen);
     return z;
   }
   (** Section 6.1 - SHA-3 Hash Functions *)
@@ -99,8 +152,6 @@ module Keccak1600 = {
     z <@ keccak1600(512, m++[true; true], d);
     return z;
   }
-
-
 }.
 
 
