fips202/properties/Keccak1600_Spec.ec
@@ -3,7 +3,7 @@
 
    Properties of the Keccak1600 specification.
 
-    - function byte-based specification
+    - functionol byte-based specification
     - correctness wrt imperative spec [FIPS202_SHA3.ec]
 
 ******************************************************************************)
@@ -12,22 +12,14 @@ require import AllCore List Int IntDiv.
 require StdOrder.
 import StdOrder.IntOrder.
 
+require import Keccakf1600_Spec.
+require import FIPS202_SHA3_Spec.
+
 require BitEncoding.
 import BitEncoding.BitChunking.
 
-require export FIPS202_SHA3.
-
-require import Keccakf1600_Spec.
-
 import EclibExtra.
 
-(*
-
-type bit = bool.
-type bits = bool list.
-*)
-type byte = W8.t.
-type bytes = W8.t list.
 
 op bytes2state (bs: bytes): state =
  Array25.of_list W64.zero (w64L_from_bytes bs).
@@ -35,416 +27,937 @@ op bytes2state (bs: bytes): state =
 op state2bytes (st: state): bytes =
  w64L_to_bytes (to_list st).
 
-op state_set_u8 (st: state, pos: int, x: byte): state =
- st.[pos %/ 8 <- w64_set_u8 st.[pos %/ 8] (pos %% 8) x].
+lemma size_state2bytes s:
+ size (state2bytes s) = 200.
+proof.
+by rewrite size_w64L_to_bytes Array25.size_to_list.
+qed.
 
-op state_xor_u8 (st: state, pos: int, x: byte): state =
- st.[pos %/ 8 <- w64_xor_u8 st.[pos %/ 8] (pos %% 8) x].
+lemma bits2bytes2state l:
+ bits2state l = bytes2state (bytes_from_bits l).
+proof.
+by rewrite /bytes2state w64L_from_bytes_from_bits /#.
+qed.
+
+lemma state2bytes2bits s:
+ bytes_to_bits (state2bytes s) = state2bits s.
+proof.
+by rewrite /state2bytes /state2bits w64L_to_bytes_to_bits.
+qed.
+
+lemma bytes2bits2state l:
+ bits2state (bytes_to_bits l) = bytes2state l.
+proof.
+rewrite /bits2state /bytes2state tP => i Hi.
+by rewrite w64L_from_bits_from_bytes.
+qed.
+
+(* sometimes is convenient to have a byte-view of the state... *)
+(*from JExtr*) require import WArray200.
+
+abbrev stbytes (st: state) : WArray200.t =
+ WArray200.init64 ("_.[_]" st).
+abbrev stwords (st200: WArray200.t) : state =
+ Array25.init (WArray200.get64 st200).
+
+lemma stbytesK st:
+ stwords (stbytes st) = st.
+proof.
+rewrite tP => i Hi.
+rewrite initiE //= get64E /=.
+apply W8u8.wordP => k Hk.
+rewrite pack8bE //= bits8E initiE 1:/# /= initiE 1:/# /= bits8E.
+by apply W8.init_ext => x Hx /#.
+qed.
+
+lemma stwordsK st:
+ stbytes (stwords st) = st.
+proof.
+rewrite tP => i Hi.
+rewrite initiE //= initiE 1:/# /= get64E pack8bE 1:/#.
+by rewrite initiE 1:/# /= /#.
+qed.
+
+lemma stbytes_inj s1 s2:
+ stbytes s1 = stbytes s2 => s1 = s2.
+proof.
+by move=> E; rewrite -(stbytesK s1) E stbytesK.
+qed.
+
+abbrev bytes2stbytes l = WArray200.of_list l.
+
+lemma bytes2stbytesP l:
+ stwords (bytes2stbytes l) = bytes2state l.
+proof.
+apply stbytes_inj.
+rewrite stwordsK tP => i Hi.
+rewrite get_of_list // initiE //=.
+rewrite initiE 1:/# /= nth_w64L_from_bytes 1:/#.
+rewrite pack8bE 1:/# get_of_list 1:/#.
+by rewrite nth_take // 1:/# nth_drop 1..2:/# /#.
+qed.
+
+op addstbytes = WArray200.map2 W8.(`^`).
+
+lemma stbytes_addstate st1 st2:
+ stbytes (addstate st1 st2)
+ = addstbytes (stbytes st1) (stbytes st2).
+proof.
+rewrite tP => i Hi.
+by rewrite map2iE // initiE //= map2iE 1:/# !initiE /#.
+qed.
 
 
+(**************************************************************
+     Functional Byte-oriented specification of KECCAK1600
+***************************************************************)
 
+(* the padding [pad10star1] is decomposed on a start-byte (which
+ includes domain-separation bits) and a trailing bit  *)
 
-(** [state_absorb] adds [m] to the state *)
-op state_absorb (st: state, m: bytes): state =
- addstate st (bytes2state m).
+op addratebit8 r8 (st: WArray200.t) =
+ st.[r8-1 <- st.[r8-1] `^` W8.of_int 128].
 
-(** [state_squeeze] extracts [len] bytes from [st] *)
-op state_squeeze (st: state, len: int): bytes =
+op addratebit r8 (st: state) =
+ stwords (addratebit8 r8 (stbytes st)).
+
+lemma addratebitE (r8 : int) (st : state):
+ 0 < r8 && r8 <= 200 =>
+ addratebit r8 st
+ = addstate st (bytes2state (rcons (nseq (r8 - 1) W8.zero) (W8.of_int 128))).
+proof.
+move=> Hr.
+apply stbytes_inj; rewrite /addratebit stwordsK tP => i Hi.
+pose st2:= bytes2state _.
+rewrite -{-1}(stbytesK st) -(stbytesK st2) stbytes_addstate.
+rewrite get_setE 1:/# map2iE // /st2 -bytes2stbytesP !stwordsK.
+case: (i=r8-1) => E.
+ rewrite E; congr.
+ by rewrite get_of_list 1:/#
+ nth_rcons size_nseq ifF 1:/# ifT 1:/#.
+rewrite !get_of_list 1:/# nth_rcons size_nseq ler_maxr 1:/#.
+case: (i < r8-1) => C.
+ by rewrite nth_nseq /#.
+by rewrite ifF /#.
+qed.
+
+(* Absorbs a byte-list [m] into the state *)
+op stateabsorb st m = addstate st (bytes2state m).
+
+(* Absorbs all the intermediate (rate-sized) blocks *)
+op stateabsorb_iblocks (ml: bytes list) st: state =
+ foldl (fun st m => keccak_f1600_op (stateabsorb st m)) st ml.
+
+(* Absorbs the last block (where [size m < r8]) *)
+op stateabsorb_last (r8: int, m: bytes, trail: byte) st: state =
+ addratebit r8 (stateabsorb st (rcons m trail)).
+
+(* Full absorb function *)
+op ABSORB1600 (r8: int, m: bytes, trail: byte): state =
+ stateabsorb_last r8 (chunkremains r8 m) trail (stateabsorb_iblocks (chunk r8 m) st0).
+
+(* Squeezes [len] bytes from [st] *)
+op statesqueeze (st: state) (len: int) =
  take len (state2bytes st).
 
-(*
+op statesqueeze_i r8 st i =
+ statesqueeze (st_i st i) r8.
 
-(** [chunkremnant] returns the leftovers not handled by [chunk] *)
-op chunkremnant ['a] (n: int) (bs: 'a list) =
- drop (size bs %/ n * n) bs.
-*)
-
-abbrev KECCAK_F1600 = keccak_f1600_op.
-
-(** absorb intermediate blocks *)
-op state_absorb_iblocks (ml: bytes list): state =
- foldl (fun st m => KECCAK_F1600 (state_absorb st m)) st0 ml.
-
-(** [addratebit] flips the "rate bit" *)
-op addratebit (r64: int, st: state): state =
- st.[r64-1 <- w64_xor_u8 st.[r64-1] 7 (W8.of_int 128)].
-(* alternative definition... 
-op addratebit (r64: int, st: state): state =
- let w = st.[r64-1] in
- let rb = w.[63] in
- st.[r64-1 <- w.[63 <- !rb]].
-*)
-
-op keccak1600_absorb_op (r64: int, suffix: byte, m: bytes): state =
- addratebit
-  r64
-  (state_absorb (state_absorb_iblocks (chunk (8*r64) m))
-                (rcons (chunkremains (8*r64) m) suffix)).
-
-
-(** squeezes [len] bytes from [KECCAK_F1600^i(st)] *)
-op state_squeeze_i (st: state, len: int, i: int): bytes =
-  state_squeeze (iter i KECCAK_F1600 st) len.
-
-
-op keccak1600_squeeze_op (r64: int, st: state, len: int) =
+(* Full squeeze of [outlen8] bytes *)
+op SQUEEZE1600 (r8: int, st: state, outlen8: int): bytes =
  (* intermediate blocks *)
- flatten (map (state_squeeze_i st (8*r64)) (iota_ 1 (len %/ (8*r64))))
+ flatten (map (statesqueeze_i r8 st) (iota_ 1 ((outlen8-1) %/ r8)))
  (* last block *)
- ++ state_squeeze_i st (len %% (8*r64)) (len %/ (8*r64) + 1).
+ ++ statesqueeze (st_i st ((outlen8-1) %/ r8 + 1))
+                  (outlen8 - max 0 ((outlen8-1) %/ r8 * r8)).
 
+(* The Sponge construction *)
+op KECCAK1600 (r8: int, m: bytes, trail: byte, outlen8: int): bytes =
+ SQUEEZE1600 r8 (ABSORB1600 r8 m trail) outlen8.
 
+(** DOMAIN-SEPARATION bits *)
+(* Remark: DS_BYTE includes first bit of [pad10star1] *)
+op SHA_DS_BYTE = W8.of_int 06.
+op SHAKE_DS_BYTE = W8.of_int 31.
+op RAWSHAKE_DS_BYTE = W8.of_int 07.
 
-
-op keccak1600_op (r64: int, suffix: byte, m: bytes, len8: int): bytes =
- keccak1600_squeeze_op r64 (keccak1600_absorb_op r64 suffix m) len8.
-
-
+(* Byte-level functional specification of SHA/SHAKE family *)
 op SHA3_224 (m: bytes): bytes =
- keccak1600_op 18 (W8.of_int 06) m 28.
+ KECCAK1600 144 m SHA_DS_BYTE 28.
 op SHA3_256 (m: bytes): bytes =
- keccak1600_op 17 (W8.of_int 06) m 32.
+ KECCAK1600 136 m SHA_DS_BYTE 32.
 op SHA3_384 (m: bytes): bytes =
- keccak1600_op 13 (W8.of_int 06) m 48.
+ KECCAK1600 104 m SHA_DS_BYTE 48.
 op SHA3_512 (m: bytes): bytes =
- keccak1600_op 9 (W8.of_int 06) m 64.
-op SHAKE128 (m: bytes, len8: int): bytes =
- keccak1600_op 21 (W8.of_int 31) m len8.
-op SHAKE256 (m:bytes, len8: int): bytes =
- keccak1600_op 17 (W8.of_int 31) m len8.
-
-(** Using XOFs without explicit output len argument.
-
-    Citation from [FIPS-202, A-2 (pag. 24)]:
-
-    "By design, the output length for an XOF does not affect the bits
-    that it produces, which means that the output length is not a
-    necessary input to the function. Conceptually, the output can be
-    an infinite string, and the application/protocol/system that
-    invokes the function simply computes the desired number of initial
-    bits of that string. Consequently, when two different output
-    lengths are chosen for a common message, the two outputs are
-    closely related: the longer output is an extension of the shorter
-    output. For example, given any positive integers "d" and "e", and any
-    message "M", "Trunc_d(SHAKE128(M, d+e))" is identical to "SHAKE128(M,
-    d)". The same property holds for SHAKE256."
-
-    To support such a use, we provide functions returning the "ith" (i \in
-    [1..]) block of SHAKE128/256 for a given input.                                   *)
-
-op SHAKE128_i (m: bytes, i: int): bytes =
- drop (8*21*(i-1)) (SHAKE128 m (8*21*i)).
-
-op SHAKE256_i (m: bytes, i: int): bytes =
- drop (8*17*(i-1)) (SHAKE256 m (8*17*i)).
+ KECCAK1600 72 m SHA_DS_BYTE 64.
+op SHAKE128 (m: bytes, outlen8:int): bytes =
+ KECCAK1600 168 m SHAKE_DS_BYTE outlen8.
+op SHAKE256 (m: bytes, outlen8:int): bytes =
+ KECCAK1600 136 m SHAKE_DS_BYTE outlen8.
+op RAWSHAKE128 (m: bytes, outlen8:int): bytes =
+ KECCAK1600 168 m RAWSHAKE_DS_BYTE outlen8.
+op RAWSHAKE256 (m: bytes, outlen8:int): bytes =
+ KECCAK1600 136 m RAWSHAKE_DS_BYTE outlen8.
 
 
+(**************************************************************
+     Correctness wrt bit-oriented functional specification
+***************************************************************)
 
+op DS_BYTE_ok ds_bits ds_byte =
+ size ds_bits <= 6 /\ ds_byte = W8.bits2w (rcons ds_bits true).
 
-
-
-(*******************************************************************************
-                               Correctness proof
-*******************************************************************************)
-
-
-lemma Array25_of_listK' ['a] (d:'a) l:
- to_list (Array25.of_list d l)
- = take 25 (l ++ nseq 25 d).
+lemma SHA_DS_BYTE_ok:
+ DS_BYTE_ok SHA_DS_BITS SHA_DS_BYTE.
 proof.
-apply (eq_from_nth d).
- by rewrite size_to_list size_take; smt(size_cat size_ge0 size_nseq).
-rewrite size_to_list => i Hi.
-rewrite /Array25.to_list nth_mkseq //=.
-rewrite get_of_list // take_cat.
-case: (25 < size l) => C.
- by rewrite nth_take /#.
-rewrite nth_cat.
-case: (i < size l) => C2 //.
-by rewrite take_nseq nth_nseq; smt(nth_out size_ge0).
+rewrite /DS_BYTE_ok /SHA_DS_BYTE /SHA_DS_BITS //=.
+apply (W8.all_eq_eq).
+by rewrite /W8.of_int /int2bs /mkseq -iotaredE /all_eq /=.
 qed.
 
-print chunkfill.
-(* este faz sentido (em vez de ter de lidar com os nseqs... *)
-op chunkfill' ['a] (d:'a) n l =
- take n (l ++ nseq n d).
-
-
-lemma state2bitsK:
- cancel state2bits bits2state.
-admitted.
-
-lemma bits2stateK bs:
- state2bits (bits2state bs)
- = chunkfill' false 1600 bs.
- admitted.
-
-lemma addstateA (s1 s2 s3: state):
- addstate s1 (addstate s2 s3) = addstate (addstate s1 s2) s3.
+lemma SHAKE_DS_BYTE_ok:
+ DS_BYTE_ok SHAKE_DS_BITS SHAKE_DS_BYTE.
 proof.
-rewrite /addstate; apply ext_eq => i Hi.
-by rewrite !map2iE // W64.WRing.AddMonoid.addmA. 
+rewrite /DS_BYTE_ok /SHAKE_DS_BYTE /SHAKE_DS_BITS //=.
+apply (W8.all_eq_eq).
+by rewrite /W8.of_int /int2bs /mkseq -iotaredE /all_eq /=.
 qed.
 
-op xorbits (xs ys: bool list) = map2 Logic.(^) xs ys.
-
-lemma addstate_xorbits bs1 bs2:
- size bs1 = size bs2 =>
- addstate (bits2state bs1) (bits2state bs2)
- = bits2state (xorbits bs1 bs2).
+lemma RAWSHAKE_DS_BYTE_ok:
+ DS_BYTE_ok RAWSHAKE_DS_BITS RAWSHAKE_DS_BYTE.
 proof.
-move=> Hsz .
-rewrite /bits2state /addstate; apply Array25.ext_eq => i Hi.
-rewrite map2iE // !get_of_list //.
-rewrite !nth_w64L_from_bits /xorbits 1..3:/#  drop_map2 take_map2.
-apply W64.ext_eq => k Hk.
-rewrite !get_bits2w //.
-case: (k < size (take 64 (drop (i * 64) bs1))) => C.
- rewrite (nth_map2 false false).
-  rewrite size_take // size_drop 1:/#.
-  smt(size_take size_drop size_ge0).
- smt(W64.get_bits2w).
-rewrite nth_out; first by rewrite size_map2 1:/#.
-by rewrite xorwE !get_bits2w // !nth_take 1..4:/# !nth_drop 1..4:/# !nth_out; smt(size_take size_drop).
+rewrite /DS_BYTE_ok /RAWSHAKE_DS_BYTE /RAWSHAKE_DS_BITS //=.
+apply (W8.all_eq_eq).
+by rewrite /W8.of_int /int2bs /mkseq -iotaredE /all_eq /=.
 qed.
 
-lemma W64_bits2w_nseq0 n:
- W64.bits2w (nseq n false)
- = W64.zero.
+lemma split_padded_rcons r8 m ds_bits:
+ 0 < r8 =>
+ size ds_bits <= 6 =>
+ split_padded (8*r8) (bytes_to_bits m ++ ds_bits)
+ = rcons (chunk (8*r8) (bytes_to_bits m))
+    (chunkremains (8*r8) (bytes_to_bits m) ++ ds_bits
+     ++ pad10star1 (8*r8) (size (bytes_to_bits m ++ ds_bits))).
 proof.
-apply W64.ext_eq => i Hi.
-by rewrite /bits2w initiE //= nth_nseq_if /#.
+move=> Hr Hsz.
+rewrite -!catA chunk_cat' 1:/# -cats1 !catA; congr.
+by rewrite chunk_size 1:/# !size_cat // size_chunkremains size_pad10star1
+  1:/# size_bytes_to_bits; smt(size_ge0).
 qed.
 
-lemma addratebit_addstate r64 st:
- 0 < r64 <= 25 =>
- addratebit r64 st
- = addstate st (bits2state (rcons (nseq (64*r64-1) false) true)).
-proof.
-move=> Hr64; rewrite /addratebit /addstate /=.
-apply ext_eq => i Hi.
-rewrite map2iE //.
-case: (i = r64-1) => C; last first.
- rewrite get_setE 1:/# C /= /bits2state get_of_list //.
- rewrite nth_w64L_from_bits 1:/# -cats1.
- case (i < r64-1) => C2.
-  rewrite drop_cat size_nseq ifT 1:/# drop_nseq 1:/#.
-  rewrite take_cat ifT ?size_nseq 1:/# take_nseq. 
-  by rewrite W64_bits2w_nseq0 /#.
- rewrite drop_cat ifF ?size_nseq 1:/# drop_oversize 1:/#.
- by rewrite /= W64_bits2w_nil.
-rewrite /bits2state get_of_list // nth_w64L_from_bits 1:/# -cats1.
-rewrite get_setE 1:/# ifT 1:/#.
-apply W64.ext_eq => k Hk.
-rewrite xorwE /=.
-case: (k = 63) => C2.
- rewrite /w64_xor_u8 /= pack8wE // get_setE // C2 /=.
- rewrite nth_take // nth_drop // 1:/# nth_cat ifF.
-  by rewrite size_nseq /#.
- rewrite size_nseq C /= lez_maxr 1:/# of_intE /int2bs /mkseq -iotaredE /=.
- pose X:= (_ = 0).
- by have ->{X}/=: X=true by smt().
-rewrite /w64_xor_u8 /= pack8wE // get_setE // eq_sym.
-rewrite C drop_cat ifT ?size_nseq 1:/# drop_nseq 1:/#.
-rewrite take_cat ?size_nseq ifF 1:/#.
-pose X:= 64 - _.
-have ->{X}: X=(size [true]) by smt().
-rewrite take_size get_bits2w 1:// nth_cat ifT ?size_nseq 1:/# nth_nseq 1:/# /=.
-case: (k %/ 8 = 7) => E.
- rewrite W8u8.get_bits8 // E xorwE.
- have Emod: k %% 8 <> 7 by smt().
- have ->: (W8.of_int 128).[k %% 8] = false.
-  by rewrite of_intE /int2bs /mkseq -iotaredE /= /bits2w initiE 1:/# /= /#.
- smt().
-by rewrite get_unpack8 1:/# W8u8.get_bits8.
-qed.
-
-lemma size_pad10star1 r len:
+lemma absorb_iblocks r r8 m:
  0 < r =>
- 0 <= len %% r <= r-2 =>
- size (pad10star1 r len)
- = r - (len %% r).
+ r = 8 * r8 =>
+ foldl (fun s b => keccak_f1600_op (addstate s b))
+       st0
+       (map bits2state (chunk r (bytes_to_bits m))) 
+ = stateabsorb_iblocks (chunk r8 m) st0.
 proof.
-move=> Hr Hlen.
-rewrite /pad10star1 /= size_rcons size_nseq lez_maxr 1:/#.
-rewrite -modzDml -modzNm -modzDl /#.
+move=> Hr Er.
+rewrite /state_absorbiblocks Er.
+rewrite chunk_bytes_to_bits.
+rewrite -map_comp foldl_map.
+apply eq_foldl => //.
+move=> s l /=; congr.
+rewrite /stateabsorb; congr.
+by rewrite /(\o) /= bytes2bits2state.
 qed.
 
-(*
-lemma size_pad10star1 r len:
- 0 < r =>
- 0 <= len <= r-2 =>
- size (pad10star1 r len)
- = r - (len %% r).
+lemma keccak1600_absorb_opE r r8 m ds_bits ds_byte:
+ 0 < r <= 1600 =>
+ r = 8*r8 =>
+ DS_BYTE_ok ds_bits ds_byte =>
+ keccak1600_absorb_op r (bytes_to_bits m ++ ds_bits)
+ = keccak_f1600_op (ABSORB1600 r8 m ds_byte).
 proof.
-move=> Hr Hlen.
-by rewrite /pad10star1 /= size_rcons size_nseq lez_maxr /#.
-qed.
-*)
-
-lemma nosmt pad10star1_modr r64 len8 mbits_size:
- 0 < r64 =>
- pad10star1 (64*r64) (8*len8 + mbits_size)
- = pad10star1 (64*r64) (8 * (len8 %% (8*r64)) + mbits_size).
-proof.
-move=> Hr; rewrite /pad10star1; congr; congr; congr.
-have ->: -(8 * len8 + mbits_size) - 2 = - (8 * len8 + (mbits_size + 2)) by ring.
-rewrite -modzNm -modzDml {1}(:64*r64=8*(8*r64)) 1:/# -mulz_modr // modzNm /#.
-qed.
-
-lemma nosmt chunk_padded r64 bs mbits:
- 0 < r64 =>
- size mbits <= 6 =>
- chunk (64*r64) (bytes_to_bits bs ++ mbits ++ pad10star1 (64*r64) (8*size bs + size mbits))
- = chunk (64*r64) (bytes_to_bits bs)
-   ++ [chunkremains (64*r64) (bytes_to_bits bs) ++ mbits ++ pad10star1 (64*r64) (8*(size bs%%(8*r64)) + size mbits)].
-proof.
-move => Hr64 Hmbits; rewrite -catA chunk_cat' 1:/#; congr.
-rewrite chunk1 1:/#.
- rewrite !size_cat size_chunkremains size_bytes_to_bits size_pad10star1 1:/#; first smt(size_ge0).
- rewrite (:64*r64=8*r64*8) 1:/#.
- have [_ B]:= divmod_mul (8*r64) 8 (size bs) (size mbits) _ _; smt(size_ge0).
-by rewrite !catA; congr; congr; apply pad10star1_modr.
-qed.
-
-(*
-search chunkremains.
-lemma chunkify_cat' ['a]:
-   forall (n : int) (l1 l2 : 'a list),
-     0 < n =>
-     chunkify n (l1 ++ l2) = chunk n l1 ++ chunkify n (chunkremains n l1 ++ l2).
-*)
-(*
-lemma chunk_padded' r64 bs mbits:
- 0 < r64 =>
- size mbits <= 6 =>
- chunk (64*r64) (bytes_to_bits bs ++ mbits ++ pad10star1 (64*r64) (8*size bs + size mbits))
- = chunk (64*r64) (bytes_to_bits bs)
-   ++ [chunkremains (64*r64) (bytes_to_bits bs) ++ mbits ++ pad10star1 (64*r64) (8*size bs + size mbits)].
-proof.
-move => Hr64 Hmbits; rewrite -catA chunk_cat' 1:/#; congr.
-rewrite chunk1 1:/#.
- rewrite !size_cat size_chunkremains size_bytes_to_bits size_pad10star1 1:/#; first smt(size_ge0).
- rewrite (:64*r64=8*r64*8) 1:/#.
- have [_ B]:= divmod_mul (8*r64) 8 (size bs) (size mbits) _ _; smt(size_ge0).
-smt(catA).
-qed.
-*)
-
-lemma pad10star1_split r l n:
- 0 < r =>
- size l <= r-2 =>
- n = size  l =>
- l ++ pad10star1 r n
- = xorbits (rcons l true ++ nseq (r - size l - 1) false)
-           (rcons (nseq (r-1) false) true).
-proof.
-have Hsz_ge0 := size_ge0 <:bool>.
-move => Hr Hsz ->; apply (eq_from_nth false).
- by rewrite size_map2 !size_cat !size_rcons !size_nseq size_pad10star1 /#.
-move=> i.
-pose S:= size _; have ->{S}: S = r. 
- rewrite /S size_cat size_pad10star1 // 2:/#.
- by rewrite modz_small /#.
-move=> Hi.
-rewrite /xorbits (nth_map2 false false).
- smt(size_rcons size_nseq size_cat).
-rewrite nth_cat.
-case: (i < size l) => C1.
- rewrite -cats1 -!catA nth_cat C1 /= nth_rcons ifT.
-  by rewrite size_nseq /#.
- by rewrite nth_nseq /#.
-rewrite -cats1 -catA nth_cat C1.
-rewrite /pad10star1 /=.
-case: (i-size l<>0) => C2 /=.
- rewrite nth_nseq 1:/# addFb nth_rcons.
- have ->: ((- size l)-2) %% r = r-size l-2.
-  by rewrite -modzDl /#.
- rewrite size_nseq lez_maxr 1:/#.
- case: (i - size l - 1 < r - size l - 2) => C3;
-  smt(nth_nseq nth_rcons size_nseq).
-rewrite nth_rcons nth_nseq; smt(size_nseq size_ge0).
+move=> Hr Hr8 [Hdsbits Hdsbyte].
+rewrite /keccak1600_absorb_op /ABSORB1600.
+(* intermediate blocks *)
+rewrite Hr8 split_padded_rcons 1..2:/# map_rcons.
+rewrite foldl_rcons /= /stateabsorb_last; congr.
+rewrite (absorb_iblocks _ r8) 1..2:/#.
+(* lastblock *)
+pose ST:= stateabsorb_iblocks _ _.
+have E8: 8*size m %/ (8*r8) * (8*r8)
+        = 8*(size m %/ r8 * r8) by smt().
+rewrite /chunkremains !size_bytes_to_bits E8.
+rewrite -bytes_to_bits_drop -cats1 /stateabsorb -bytes2bits2state.
+rewrite bytes_to_bits_cat /pad10star1 -cat1s !catA -cats1 bits2state_cat addstateA !catA cat_nseq;
+ 1..2:smt(size_ge0).
+rewrite !size_cat !size_bytes_to_bits !size_drop;
+ 1: smt(size_ge0).
+rewrite ler_maxr /=; 1:smt(size_ge0).
+have ->: size m - size m %/ r8 * r8
+         = size m %% r8 by smt().
+have ->: (- (8 * size m + size ds_bits)) - 2
+         = - (8*size m + size ds_bits + 2) by smt().
+rewrite modNz //=; 1..2:smt(size_ge0).
+have ->: (8 * size m + size ds_bits + 1) %% (8 * r8)
+         = (size m * 8 + (size ds_bits + 1))%%(r8*8)
+ by smt().
+have [_ ->]:= divmod_mul r8 8 (size m) (size ds_bits+1) _ _; 1..2:smt(size_ge0).
+have ->: 8 * (size m %% r8) + size ds_bits + 1 + (8 * r8 - 1 - (size m %% r8 * 8 + (size ds_bits + 1)))
+         = 8*r8 - 1 by smt().
+rewrite addratebitE 1:/#; congr.
+ congr. 
+ rewrite bits2bytes2state -catA bytes_from_bits_cat.
+  by rewrite size_bytes_to_bits /#.
+ rewrite bytes_to_bitsK -bytes_to_bits_cat bits2bytes2state bytes_to_bitsK; congr; congr.
+ rewrite bytes_from_bits_cons.
+  rewrite size_cat; smt(size_ge0).
+ by rewrite take_oversize 1:size_cat // 1:/# drop_oversize 1:size_cat 1:/# bytes_from_bits_nil cats1 /#.
+rewrite bits2bytes2state; congr.
+rewrite (:8*r8-1=8*(r8-1)+7) 1:/#.
+rewrite -cat_nseq // 1:/# -catA -cats1.
+rewrite bytes_from_bits_cat.
+ by rewrite size_nseq ler_maxr /#.
+congr.
+ by rewrite bytes_from_bits_nseq0 /#.
+rewrite -mkseq_nseq /mkseq -iotaredE /= /bytes_from_bits chunkify_chunk // chunk_size //=. 
+apply W8.all_eq_eq; rewrite /all_eq /=.
+by rewrite of_intE /int2bs /mkseq -iotaredE /=.
 qed.
 
-(*
-op keccak1600_absorb_op (r64: int, suffix: byte, m: bytes): state =
- addratebit
-  r64
-  (state_absorb (state_absorb_iblocks r64 m)
-                (rcons (chunkremains (8*r64) m) suffix)).
-*)
-lemma bits2state_cat_nseq0 n bs:
- bits2state (bs ++ nseq n false) = bits2state bs.
+lemma keccak1600_squeeze_opE r r8 st outlen outlen8:
+ 0 < r <= 1600 =>
+ r = 8*r8 =>
+ outlen = 8*outlen8 =>
+ keccak1600_squeeze_op r (keccak_f1600_op st) outlen
+ = bytes_to_bits (SQUEEZE1600 r8 st outlen8).
 proof.
-rewrite /bits2state.
-admit.
+move=> Hr Hr8 Ho8.
+case: (outlen <= 0) => Hout.
+ rewrite /keccak1600_squeeze_op take_le0 1:/# //.
+ rewrite /SQUEEZE1600 iota0 1:/#  flatten_nil /=.
+ by rewrite /statesqueeze take_le0 /#.
+rewrite /keccak1600_squeeze_op /SQUEEZE1600.
+rewrite bytes_to_bits_cat iotaSr 1:/#.
+rewrite map_rcons flatten_rcons take_cat.
+pose ll:= flatten _.
+have size_ll: size ll = (outlen - 1) %/ r * r.
+ rewrite (size_flatten' r).
+  move=> x /mapP [y [Hy]].
+  rewrite /(\o) /= => ->.
+  by rewrite size_take' 1:/# ifT ?size_state2bits 1:/#.
+ by rewrite size_map /(\o) /= size_iota ler_maxr /#.
+rewrite ifF ?size_ll 1:/#.
+have E: (outlen - 1) %/ r = (outlen8-1) %/ r8.
+ by rewrite Ho8 mulrC Hr8 divzMr // 1:/# divzMDl //=.
+congr.
+ rewrite (:iota_ 1 = iota_ (1+0)) 1:/# iota_addl -map_comp.
+ rewrite /ll E bytes_to_bits_flatten; congr.
+ rewrite -map_comp.
+ apply eq_in_map => x /@mem_iota /> *.
+ rewrite /(\o) /= /statesqueeze_i addrC /state_squeeze bytes_to_bits_take; congr.
+ rewrite state2bytes2bits; congr.
+ by rewrite /st_i iterSr //.
+pose L:=outlen - _.
+rewrite /statesqueeze bytes_to_bits_take.
+rewrite /(\o) /= state2bytes2bits.
+rewrite take_take'; congr.
+ rewrite /L ler_maxr 1:/#.
+ by rewrite ler_minl /#.
+congr.
+rewrite /st_i.
+have ->: (outlen - 1) %/ r = (outlen8-1) %/ r8.
+ by rewrite Ho8 mulrC Hr8 divzMr // 1:/# divzMDl //=.
+by rewrite iterSr /#.
 qed.
 
-lemma bits2bytes2state bs:
- bits2state bs = bytes2state (bytes_from_bits bs).
-admitted.
-
-lemma addstate_last (st:state) r64 mbits bs suffix:
- 0 < r64 <= 25 =>
- size mbits <= 6 =>
- suffix = W8.bits2w (rcons mbits true) =>
- addstate st (bits2state (chunkremains (64*r64) (bytes_to_bits bs) ++ mbits ++ pad10star1 (64*r64) (8*(size bs %% (8*r64)) + size mbits)))
- = addratebit r64 (addstate st (bytes2state (rcons (chunkremains (8*r64) bs) suffix))).
+lemma keccak1600_opE c r8 m ds_bits ds_byte outlen outlen8:
+ 0 <= c < 1600 =>
+ 1600 - c = 8*r8 =>
+ outlen = 8*outlen8 =>
+ DS_BYTE_ok ds_bits ds_byte =>
+ keccak1600_op c (bytes_to_bits m ++ ds_bits) outlen
+ = bytes_to_bits (KECCAK1600 r8 m ds_byte outlen8).
 proof.
-move=> Hr64 Hmbits Hsuffix.
-rewrite pad10star1_split 1:/#.
-  by rewrite size_cat size_chunkremains size_bytes_to_bits /#.
- by rewrite size_cat size_chunkremains size_bytes_to_bits /#.
-rewrite -addstate_xorbits. 
- rewrite size_cat !size_rcons !size_cat !size_nseq size_chunkremains size_bytes_to_bits; smt(size_ge0).
-rewrite addstateA -addratebit_addstate //; congr; congr.
-rewrite bits2state_cat_nseq0 -(bits2state_cat_nseq0 (7-size mbits)) bits2bytes2state.
-pose L := _ ++ _.
-have ->: L = bytes_to_bits (rcons (chunkremains (8 * r64) bs) suffix).
- rewrite /L -!cats1 bytes_to_bits_cat /chunkremains bytes_to_bits_drop -!catA; congr.
-  by congr; rewrite size_bytes_to_bits /#.
- rewrite !catA bytes_to_bits_cons bytes_to_bits_nil cats0.
- rewrite Hsuffix W8_bits2wK' ?size_rcons 1:/# cats1; congr; smt().
-by rewrite bytes_to_bitsK.
+move=> *; rewrite /KECCAK1600 /keccak1600_op /keccak1600_sponge_op.
+rewrite (keccak1600_absorb_opE _ r8 _ _ ds_byte) // 1:/#.
+by apply keccak1600_squeeze_opE => // /#.
+qed.
+
+lemma sha3_224_opE m:
+ sha3_224_op (bytes_to_bits m)
+ = bytes_to_bits (SHA3_224 m).
+proof.
+apply keccak1600_opE => //.
+exact SHA_DS_BYTE_ok.
+qed.
+
+lemma sha3_256_opE m:
+ sha3_256_op (bytes_to_bits m)
+ = bytes_to_bits (SHA3_256 m).
+proof.
+apply keccak1600_opE => //.
+exact SHA_DS_BYTE_ok.
+qed.
+
+lemma sha3_384_opE m:
+ sha3_384_op (bytes_to_bits m)
+ = bytes_to_bits (SHA3_384 m).
+proof.
+apply keccak1600_opE => //.
+exact SHA_DS_BYTE_ok.
+qed.
+
+lemma sha3_512_opE m:
+ sha3_512_op (bytes_to_bits m)
+ = bytes_to_bits (SHA3_512 m).
+proof.
+apply keccak1600_opE => //.
+exact SHA_DS_BYTE_ok.
+qed.
+
+lemma shake128_opE m outlen outlen8:
+ outlen = 8*outlen8 =>
+ shake128_op (bytes_to_bits m) outlen
+ = bytes_to_bits (SHAKE128 m outlen8).
+proof.
+move=> H; apply keccak1600_opE => //.
+exact SHAKE_DS_BYTE_ok.
+qed.
+
+lemma shake256_opE m outlen outlen8:
+ outlen = 8*outlen8 =>
+ shake256_op (bytes_to_bits m) outlen
+ = bytes_to_bits (SHAKE256 m outlen8).
+proof.
+move=> H; apply keccak1600_opE => //.
+exact SHAKE_DS_BYTE_ok.
+qed.
+
+lemma rawshake128_opE m outlen outlen8:
+ outlen = 8*outlen8 =>
+ rawshake128_op (bytes_to_bits m) outlen
+ = bytes_to_bits (RAWSHAKE128 m outlen8).
+proof.
+move=> H; apply keccak1600_opE => //.
+exact RAWSHAKE_DS_BYTE_ok.
+qed.
+
+lemma rawshake256_opE m outlen outlen8:
+ outlen = 8*outlen8 =>
+ rawshake256_op (bytes_to_bits m) outlen
+ = bytes_to_bits (RAWSHAKE256 m outlen8).
+proof.
+move=> H; apply keccak1600_opE => //.
+exact RAWSHAKE_DS_BYTE_ok.
 qed.
 
 
-lemma nth_chunk ['a] k (l: 'a list) i:
- 0 < k =>
- k %| size l =>
- nth [] (chunk k l) i =
- take k (drop (k*i) l).
+(**************************************************************
+     Correctness of (bit-level) FIPS202 standard
+   wrt byte-level functional spec.
+***************************************************************)
+
+hoare fips202_KECCAK1600_h _ds_bits _r8 _ds_byte _m _outlen8:
+ Keccak1600.keccak1600
+ : c = 1600 - 8*_r8 /\
+   0 < _r8 <= 200 /\
+   m = bytes_to_bits _m ++ _ds_bits /\
+   DS_BYTE_ok _ds_bits _ds_byte /\
+   outlen = 8*_outlen8
+   ==> res = bytes_to_bits (KECCAK1600 _r8 _m _ds_byte _outlen8).
 proof.
-admitted.
-
-
-print Keccak1600.
-(*
-  proc sponge1600_pad10star1(r : int, m : bool list, d : int) : bool list = {
-*)
-
-
-lemma sponge_correct _r64 _m _suffix _mbits _len8:
- 0 < _len8 => (* this can be removed by an extra case... *)
- size _mbits <= 6 =>
- W8.w2bits _suffix = rcons _mbits true =>
- hoare [ Keccak1600.sponge1600_pad10star1:
-         r = 64*_r64 /\ m = bytes_to_bits _m ++ _mbits /\ d = 8*_len8
-         ==> res = bytes_to_bits (keccak1600_op _r64 _suffix _m _len8 )].
-proof.
-move=> Hlen8 Hmbits Hsuffix; proc; simplify.
-seq 6: (#pre /\ s = keccak1600_absorb_op _r64 _suffix _m).
-print keccak1600_absorb_op.
- while (#pre /\ n = size m %/ 8 + 1 /\ 0 <= i <= n /\
-        pl = chunk r (bytes_to_bits _m ++ _mbits ++ pad10star1 r (8 * (size _m) + size _mbits)) /\
-        s <- state_absorb_iblocks r64 
- admit.
-exlim (keccak1600_absorb_op _r64 _suffix _m) => st.
-splitwhile 2: (size z + d < d).
-seq 2: (#[:-2]pre /\ s = (iter (d %/ r) KECCAK_F1600 st) /\ size z = r * (d %/ r)) => //.
- admit.
-admit.
+conseq (keccak1600_h (1600-8*_r8) (bytes_to_bits _m++_ds_bits) (8*_outlen8)).
+ by move=> &m H => /> /#.
+smt(keccak1600_opE).
 qed.
+
+phoare fips202_KECCAK1600_ph _ds_bits _r8 _ds_byte _m _outlen8:
+ [ Keccak1600.keccak1600
+ : c = 1600 - 8*_r8 /\
+   0 < _r8 <= 200 /\
+   m = bytes_to_bits _m ++ _ds_bits /\
+   DS_BYTE_ok _ds_bits _ds_byte /\
+   outlen = 8*_outlen8
+   ==> res = bytes_to_bits (KECCAK1600 _r8 _m _ds_byte _outlen8)
+ ] = 1%r.
+proof.
+by conseq keccak1600_ll (fips202_KECCAK1600_h _ds_bits _r8 _ds_byte _m _outlen8) => /#.
+qed.
+
+hoare fips202_SHA3_224_h _m:
+ Keccak1600.sha3_224
+ : m = bytes_to_bits _m ==> res = bytes_to_bits (SHA3_224 _m).
+proof.
+conseq (sha3_224_h (bytes_to_bits _m)).
+smt(sha3_224_opE).
+qed.
+
+phoare fips202_SHA3_224_ph _m:
+ [ Keccak1600.sha3_224
+ : m = bytes_to_bits _m ==> res = bytes_to_bits (SHA3_224 _m)
+ ] = 1%r.
+proof.
+have Hll: islossless Keccak1600.sha3_224 by proc; call keccak1600_ll.
+by conseq Hll (fips202_SHA3_224_h _m).
+qed.
+
+hoare fips202_SHA3_256_h _m:
+ Keccak1600.sha3_256
+ : m = bytes_to_bits _m ==> res = bytes_to_bits (SHA3_256 _m).
+proof.
+conseq (sha3_256_h (bytes_to_bits _m)).
+smt(sha3_256_opE).
+qed.
+
+phoare fips202_SHA3_256_ph _m:
+ [ Keccak1600.sha3_256
+ : m = bytes_to_bits _m ==> res = bytes_to_bits (SHA3_256 _m)
+ ] = 1%r.
+proof.
+have Hll: islossless Keccak1600.sha3_256 by proc; call keccak1600_ll.
+by conseq Hll (fips202_SHA3_256_h _m).
+qed.
+
+hoare fips202_SHA3_384_h _m:
+ Keccak1600.sha3_384
+ : m = bytes_to_bits _m ==> res = bytes_to_bits (SHA3_384 _m).
+proof.
+conseq (sha3_384_h (bytes_to_bits _m)).
+smt(sha3_384_opE).
+qed.
+
+phoare fips202_SHA3_384_ph _m:
+ [ Keccak1600.sha3_384
+ : m = bytes_to_bits _m ==> res = bytes_to_bits (SHA3_384 _m)
+ ] = 1%r.
+proof.
+have Hll: islossless Keccak1600.sha3_384 by proc; call keccak1600_ll.
+by conseq Hll (fips202_SHA3_384_h _m).
+qed.
+
+hoare fips202_SHA3_512_bh _m:
+ Keccak1600.sha3_512
+ : m = bytes_to_bits _m ==> res = bytes_to_bits (SHA3_512 _m).
+proof.
+conseq (sha3_512_h (bytes_to_bits _m)).
+smt(sha3_512_opE).
+qed.
+
+phoare fips202_SHA3_512_ph _m:
+ [ Keccak1600.sha3_512
+ : m = bytes_to_bits _m ==> res = bytes_to_bits (SHA3_512 _m)
+ ] = 1%r.
+proof.
+have Hll: islossless Keccak1600.sha3_512 by proc; call keccak1600_ll.
+by conseq Hll (fips202_SHA3_512_bh _m).
+qed.
+
+hoare fips202_SHAKE128_h _m _len8:
+ Keccak1600.shake128
+ : m = bytes_to_bits _m /\ d = 8*_len8 
+   ==> res = bytes_to_bits (SHAKE128 _m _len8).
+proof.
+conseq (shake128_h (bytes_to_bits _m) (8*_len8)).
+smt(shake128_opE).
+qed.
+
+phoare fips202_SHAKE128_ph _m _len8:
+ [ Keccak1600.shake128
+ : m = bytes_to_bits _m /\ d = 8*_len8 
+   ==> res = bytes_to_bits (SHAKE128 _m _len8)
+ ] = 1%r.
+proof.
+have Hll: islossless Keccak1600.shake128 by proc; call keccak1600_ll.
+by conseq Hll (fips202_SHAKE128_h _m _len8).
+qed.
+
+hoare fips202_SHAKE256_h _m _len8:
+ Keccak1600.shake256
+ : m = bytes_to_bits _m /\ d = 8*_len8 
+   ==> res = bytes_to_bits (SHAKE256 _m _len8).
+proof.
+conseq (shake256_h (bytes_to_bits _m) (8*_len8)).
+smt(shake256_opE).
+qed.
+
+phoare fips202_SHAKE256_ph _m _len8:
+ [ Keccak1600.shake256
+ : m = bytes_to_bits _m /\ d = 8*_len8 
+   ==> res = bytes_to_bits (SHAKE256 _m _len8)
+ ] = 1%r.
+proof.
+have Hll: islossless Keccak1600.shake256 by proc; call keccak1600_ll.
+by conseq Hll (fips202_SHAKE256_h _m _len8).
+qed.
+
+hoare fips202_RAWSHAKE128_h _m _len8:
+ Keccak1600.rawSHAKE128
+ : m = bytes_to_bits _m /\ d = 8*_len8 
+   ==> res = bytes_to_bits (RAWSHAKE128 _m _len8).
+proof.
+conseq (rawshake128_h (bytes_to_bits _m) (8*_len8)).
+smt(rawshake128_opE).
+qed.
+
+phoare fips202_RAWSHAKE128_ph _m _len8:
+ [ Keccak1600.rawSHAKE128
+ : m = bytes_to_bits _m /\ d = 8*_len8 
+   ==> res = bytes_to_bits (RAWSHAKE128 _m _len8)
+ ] = 1%r.
+proof.
+have Hll: islossless Keccak1600.rawSHAKE128 by proc; call keccak1600_ll.
+by conseq Hll (fips202_RAWSHAKE128_h _m _len8).
+qed.
+
+hoare fips202_RAWSHAKE256_h _m _len8:
+ Keccak1600.rawSHAKE256
+ : m = bytes_to_bits _m /\ d = 8*_len8 
+   ==> res = bytes_to_bits (RAWSHAKE256 _m _len8).
+proof.
+conseq (rawshake256_h (bytes_to_bits _m) (8*_len8)).
+smt(rawshake256_opE).
+qed.
+
+phoare fips202_RAWSHAKE256_ph _m _len8:
+ [ Keccak1600.rawSHAKE256
+ : m = bytes_to_bits _m /\ d = 8*_len8 
+   ==> res = bytes_to_bits (RAWSHAKE256 _m _len8)
+ ] = 1%r.
+proof.
+have Hll: islossless Keccak1600.rawSHAKE256 by proc; call keccak1600_ll.
+by conseq Hll (fips202_RAWSHAKE256_h _m _len8).
+qed.
+
+(**************************************************************
+     Imperative byte-oriented SPONGE construction
+  (a convenient target for implementation correctness proofs)
+***************************************************************)
+
+module Keccak1600Bytes = {
+ proc absorb(r8: int, inp: bytes, trail: byte): state = {
+    var l, lastb, st, i;
+    l <- chunk r8 inp;
+    st <- st0;
+    i <- 0;
+    while (i < size l) {
+      st <- stateabsorb st (nth [] l i);
+      st <- keccak_f1600_op st;
+      i <- i + 1;
+    }
+    lastb <- chunkremains r8 inp;
+    st <- stateabsorb st (rcons lastb trail);
+    st <- addratebit r8 st;
+  return st;
+ }
+ proc squeeze(r8: int, st: state, outlen: int): bytes = {
+   var out_bytes, i;
+   out_bytes <- [];
+   i <- 1;
+   st <- keccak_f1600_op st;
+   while (r8*i < outlen) {
+     out_bytes <- out_bytes ++ statesqueeze st r8;  
+     st <- keccak_f1600_op st;
+     i <- i + 1;
+   }
+   out_bytes <- out_bytes ++ statesqueeze st (outlen - r8*(i-1));
+   return out_bytes;
+ }
+ proc sponge(r8:int, m: bytes, trail: byte, len8: int): bytes = {
+   var s, r;
+   s <@ absorb(r8, m, trail);
+   r <@ squeeze(r8, s, len8);
+  return r;
+ }
+ proc sha3_224(m: bytes): bytes = {
+   var r;
+   r <@ sponge(144, m, SHA_DS_BYTE, 28);
+   return r;
+ }
+ proc sha3_256(m: bytes): bytes = {
+   var r;
+   r <@ sponge(136, m, SHA_DS_BYTE, 32);
+   return r;
+ }
+ proc sha3_384(m: bytes): bytes = {
+   var r;
+   r <@ sponge(104, m, SHA_DS_BYTE, 48);
+   return r;
+ }
+ proc sha3_512(m: bytes): bytes = {
+   var r;
+   r <@ sponge(72, m, SHA_DS_BYTE, 64);
+   return r;
+ }
+ proc shake128(m: bytes, outlen8: int): bytes = {
+   var r;
+   r <@ sponge(168, m, SHAKE_DS_BYTE, outlen8);
+   return r;
+ }
+ proc shake256(m: bytes, outlen8: int): bytes = {
+   var r;
+   r <@ sponge(136, m, SHAKE_DS_BYTE, outlen8);
+   return r;
+ }
+ proc rawshake128(m: bytes, outlen8: int): bytes = {
+   var r;
+   r <@ sponge(168, m, RAWSHAKE_DS_BYTE, outlen8);
+   return r;
+ }
+ proc rawshake256(m: bytes, outlen8: int): bytes = {
+   var r;
+   r <@ sponge(136, m, RAWSHAKE_DS_BYTE, outlen8);
+   return r;
+ }
+}.
+
+hoare ABSORB1600_h _r8 _trail _m:
+ Keccak1600Bytes.absorb: r8=_r8 /\ trail=_trail /\ inp=_m /\ 0 < _r8 ==> res = ABSORB1600 _r8 _m _trail.
+proof.
+proc; simplify.
+sp 1; seq 3: (#pre /\ st = stateabsorb_iblocks l st0).
+ while (#pre /\ 0 <= i <= size l /\
+        stateabsorb_iblocks l st0
+        = stateabsorb_iblocks (drop i l) st).
+  auto => /> &m Hr Hi0 Hi1 IH.
+  rewrite size_chunk // => H; split; first smt().
+  rewrite IH dropS 1:/#.
+  rewrite -(head_behead (drop i{m} _) []) /=. 
+   by rewrite -size_eq0 size_drop // size_chunk // /#.
+  rewrite /stateabsorb_iblocks /=.
+  apply eq_foldl => //.
+  rewrite /C nth_chunk // 1:/#. 
+  congr; congr.
+  rewrite drop_chunk // -nth0_head nth_chunk //=.
+   by rewrite size_drop 1:/# ler_maxr /#.
+  by rewrite drop0.
+ auto => /> *; split.
+  by rewrite size_chunk // drop0; smt(size_ge0).
+ move=> i st Hi1 _ Hi2.
+ have ->: i=size (chunk _r8 _m) by smt().
+ by rewrite drop_oversize // /#.
+by auto.
+qed.
+
+lemma ABSORB1600_ll:
+ phoare [ Keccak1600Bytes.absorb: 0 < r8 ==> true ] = 1%r.
+proof.
+proc; sp 1; simplify.
+wp; while (#pre /\ i <= size l) (size l - i).
+ by move=> z; auto => /> &m Hr /#.
+by auto => /> &m Hr; smt(size_ge0).
+qed.
+
+phoare ABSORB1600_ph _r8 _trail _m:
+ [ Keccak1600Bytes.absorb
+ : r8=_r8 /\ trail=_trail /\ inp=_m /\ 0 < _r8 
+ ==> res = ABSORB1600 _r8 _m _trail
+ ] = 1%r.
+proof. by conseq ABSORB1600_ll (ABSORB1600_h _r8 _trail _m). qed.
+
+hoare SQUEEZE1600_h _r8 _st _len:
+ Keccak1600Bytes.squeeze
+ : r8=_r8 /\ st=_st /\ outlen=_len 
+   /\ 0 < _r8 <= 200
+   ==> res = SQUEEZE1600 _r8 _st _len.
+proof.
+proc; case: (0 < outlen); simplify.
+ seq 4: (#[/1,3:]pre /\ 
+         out_bytes = flatten (map (statesqueeze_i _r8 _st) (iota_ 1 ((_len-1) %/ _r8))) /\
+         st = st_i _st ((_len-1) %/ _r8+1) /\
+         i = (_len-1) %/ _r8 + 1).
+  while (0 < i <= (_len-1) %/ _r8 + 1 /\
+         #[/1,3:]pre /\
+         out_bytes = flatten (map (statesqueeze_i _r8 _st) (iota_ 1 (i-1))) /\
+         st = st_i _st i).
+   auto => /> &m Hi_1 Hi_2 Hr8_1 Hr8_2 *; split; 1:smt().
+   split.
+    rewrite {3}(:i{m}=i{m}-1+1) 1:/# iotaSr 1:/# /=.
+    rewrite map_rcons flatten_rcons; congr.
+    by rewrite /statesqueeze_i; congr; smt().
+   by rewrite /st_i !iterS /#.
+  auto => /> *; split. 
+   by rewrite iota0 //= flatten_nil /st_i iter1 /#.
+  move => /> i???.
+  by have ->//: i=(_len-1)%/_r8+1 by smt().
+ auto => /> Hr64_1 Hr64_2 ?.
+ rewrite /SQUEEZE1600 ler_maxr 1:/#; congr; congr.
+ by rewrite mulzC {1}(divz_eq (_len-1) _r8) /#.
+rcondf 4; first by auto => /> /#.
+auto => /> *.
+rewrite /SQUEEZE1600 iota0 1:/# flatten_nil /=.
+by rewrite /statesqueeze !take_le0 /#.
+qed.
+
+lemma SQUEEZE1600_ll:
+ phoare [ Keccak1600Bytes.squeeze: 0 < r8 ==> true ] = 1%r.
+proof.
+proc; wp; simplify. 
+case: (outlen<0).
+ by rcondf 4; auto => /> /#. 
+while (0 < r8 /\ 0 < r8*i<=outlen+r8) (outlen - i).
+ move=> z; auto => /> &m Hr /#.
+by auto => /> &m Hr ? /#.
+qed.
+
+phoare SQUEEZE1600_ph _r8 _st _len:
+ [ Keccak1600Bytes.squeeze
+ : r8=_r8 /\ st=_st /\ outlen=_len /\ 0<_r8 <= 200
+   ==> res = SQUEEZE1600 _r8 _st _len
+ ] = 1%r.
+proof.
+by conseq SQUEEZE1600_ll (SQUEEZE1600_h _r8 _st _len).
+qed.
+
+hoare KECCAK1600_h _r8 _trail _m _len8:
+ Keccak1600Bytes.sponge
+ : r8=_r8 /\ trail=_trail /\ m=_m /\ len8=_len8 
+   /\ 0 < _r8 <= 200
+   ==> res = KECCAK1600 _r8 _m _trail _len8.
+proof.
+proc.
+ecall (SQUEEZE1600_h r8 s len8).
+ecall (ABSORB1600_h r8 trail m).
+by auto => />.
+qed.
+
+phoare KECCAK1600_ll:
+ [ Keccak1600Bytes.sponge: 0 < r8 ==> true ] = 1%r.
+proof.
+proc.
+call SQUEEZE1600_ll.
+call ABSORB1600_ll.
+by auto => />.
+qed.
+
+phoare KECCAK1600_ph _r8 _trail _m _len8:
+ [ Keccak1600Bytes.sponge
+   : r8=_r8 /\ trail=_trail /\ m=_m /\ len8=_len8 
+     /\ 0 < _r8 <= 200
+     ==> res = KECCAK1600 _r8 _m _trail _len8
+ ] = 1%r.
+proof. by conseq KECCAK1600_ll (KECCAK1600_h _r8 _trail _m _len8). qed.
+
+hoare SHA3_224_h _m:
+ Keccak1600Bytes.sha3_224
+ : m = _m
+   ==> res = SHA3_224 _m.
+proof. by proc; ecall (KECCAK1600_h 144 SHA_DS_BYTE m 28). qed.
+
+lemma SHA3_224_ll: islossless Keccak1600Bytes.sha3_224.
+proof. by proc; call KECCAK1600_ll. qed.
+
+phoare SHA3_224_ph _m:
+ [ Keccak1600Bytes.sha3_224
+   : m = _m
+     ==> res = SHA3_224 _m
+ ] = 1%r.
+proof. by conseq SHA3_224_ll (SHA3_224_h _m). qed.
+
+hoare SHA3_256_h _m:
+ Keccak1600Bytes.sha3_256
+ : m = _m
+   ==> res = SHA3_256 _m.
+proof. by proc; ecall (KECCAK1600_h 136 SHA_DS_BYTE m 32). qed.
+
+lemma SHA3_256_ll: islossless Keccak1600Bytes.sha3_256.
+proof. by proc; call KECCAK1600_ll. qed.
+
+phoare SHA3_256_ph _m:
+ [ Keccak1600Bytes.sha3_256
+   : m = _m
+     ==> res = SHA3_256 _m
+ ] = 1%r.
+proof. by conseq SHA3_256_ll (SHA3_256_h _m). qed.
+
+hoare SHA3_384_h _m:
+ Keccak1600Bytes.sha3_384
+ : m = _m
+   ==> res = SHA3_384 _m.
+proof. by proc; ecall (KECCAK1600_h 104 SHA_DS_BYTE m 48). qed.
+
+lemma SHA3_384_ll: islossless Keccak1600Bytes.sha3_384.
+proof. by proc; call KECCAK1600_ll. qed.
+
+phoare SHA3_384_ph _m:
+ [ Keccak1600Bytes.sha3_384
+   : m = _m
+     ==> res = SHA3_384 _m
+ ] = 1%r.
+proof. by conseq SHA3_384_ll (SHA3_384_h _m). qed.
+
+hoare SHA3_512_h _m:
+ Keccak1600Bytes.sha3_512
+ : m = _m
+   ==> res = SHA3_512 _m.
+proof. by proc; ecall (KECCAK1600_h 72 SHA_DS_BYTE m 64). qed.
+
+lemma SHA3_512_ll: islossless Keccak1600Bytes.sha3_512.
+proof. by proc; call KECCAK1600_ll. qed.
+
+phoare SHA3_512_ph _m:
+ [ Keccak1600Bytes.sha3_512
+   : m = _m
+     ==> res = SHA3_512 _m
+ ] = 1%r.
+proof. by conseq SHA3_512_ll (SHA3_512_h _m). qed.
+
+hoare SHAKE128_h _m _outlen8:
+ Keccak1600Bytes.shake128
+ : m = _m /\ outlen8=_outlen8
+   ==> res = SHAKE128 _m _outlen8.
+proof. by proc; ecall (KECCAK1600_h 168 SHAKE_DS_BYTE m outlen8). qed.
+
+lemma SHAKE128_ll: islossless Keccak1600Bytes.shake128.
+proof. by proc; call KECCAK1600_ll. qed.
+
+phoare SHAKE128_ph _m _outlen8:
+ [ Keccak1600Bytes.shake128
+   : m = _m /\ outlen8 = _outlen8
+     ==> res = SHAKE128 _m _outlen8
+ ] = 1%r.
+proof. by conseq SHAKE128_ll (SHAKE128_h _m _outlen8). qed.
+
+hoare SHAKE256_h _m _outlen8:
+ Keccak1600Bytes.shake256
+ : m = _m /\ outlen8=_outlen8
+   ==> res = SHAKE256 _m _outlen8.
+proof. by proc; ecall (KECCAK1600_h 136 SHAKE_DS_BYTE m outlen8). qed.
+
+lemma SHAKE256_ll: islossless Keccak1600Bytes.shake256.
+proof. by proc; call KECCAK1600_ll. qed.
+
+phoare SHAKE256_ph _m _outlen8:
+ [ Keccak1600Bytes.shake256
+   : m = _m /\ outlen8 = _outlen8
+     ==> res = SHAKE256 _m _outlen8
+ ] = 1%r.
+proof. by conseq SHAKE256_ll (SHAKE256_h _m _outlen8). qed.
+
+hoare RAWSHAKE128_h _m _outlen8:
+ Keccak1600Bytes.rawshake128
+ : m = _m /\ outlen8=_outlen8
+   ==> res = RAWSHAKE128 _m _outlen8.
+proof. by proc; ecall (KECCAK1600_h 168 RAWSHAKE_DS_BYTE m outlen8). qed.
+
+lemma RAWSHAKE128_ll: islossless Keccak1600Bytes.rawshake128.
+proof. by proc; call KECCAK1600_ll. qed.
+
+phoare RAWSHAKE128_ph _m _outlen8:
+ [ Keccak1600Bytes.rawshake128
+   : m = _m /\ outlen8 = _outlen8
+     ==> res = RAWSHAKE128 _m _outlen8
+ ] = 1%r.
+proof. by conseq RAWSHAKE128_ll (RAWSHAKE128_h _m _outlen8). qed.
+
+hoare RAWSHAKE256_h _m _outlen8:
+ Keccak1600Bytes.rawshake256
+ : m = _m /\ outlen8=_outlen8
+   ==> res = RAWSHAKE256 _m _outlen8.
+proof. by proc; ecall (KECCAK1600_h 136 RAWSHAKE_DS_BYTE m outlen8). qed.
+
+lemma RAWSHAKE256_ll: islossless Keccak1600Bytes.rawshake256.
+proof. by proc; call KECCAK1600_ll. qed.
+
+phoare RAWSHAKE256_ph _m _outlen8:
+ [ Keccak1600Bytes.rawshake256
+   : m = _m /\ outlen8 = _outlen8
+     ==> res = RAWSHAKE256 _m _outlen8
+ ] = 1%r.
+proof. by conseq RAWSHAKE256_ll (RAWSHAKE256_h _m _outlen8). qed.
 
 
 
