fips202/properties/FIPS202_SHA3_Spec.ec
@@ -1,0 +1,450 @@
+(******************************************************************************
+   Keccak1600_Spec.ec:
+
+   Properties of the Keccak1600 specification.
+
+    - functionol (bit-oriented) specification
+    - correctness wrt imperative spec [FIPS202_SHA3.ec]
+
+******************************************************************************)
+require import AllCore List Int IntDiv.
+
+require export FIPS202_SHA3.
+
+require import Keccakf1600_Spec.
+
+import EclibExtra JWordList.
+
+
+
+require StdOrder.
+import StdOrder.IntOrder.
+
+require BitEncoding.
+import BitEncoding.BitChunking.
+
+
+(** Auxiliary defs *)
+
+lemma size_state2bits s:
+ size (state2bits s) = 1600.
+proof.
+by rewrite /state2bits size_w64L_to_bits size_to_list /#.
+qed.
+
+lemma bits2state_cat l1 l2:
+ bits2state (l1++l2)
+ = addstate (bits2state l1)
+            (bits2state (nseq (size l1) false ++ l2)).
+proof.
+apply Array25.ext_eq => i Hi.
+rewrite map2iE // !get_of_list //.
+rewrite !nth_w64L_from_bits 1..3:/#.
+apply W64.wordP => k Hk.
+rewrite xorE map2iE // !get_bits2w //.
+rewrite !nth_take 1..6:/# !nth_drop 1..6:/#.
+rewrite !nth_cat size_nseq ler_maxr; 1:smt(size_ge0).
+case: (64*i+k < size l1) => C.
+ by rewrite nth_nseq /#.
+by rewrite (nth_out _ l1) /#.
+qed.
+
+lemma addstateA (s1 s2 s3: state):
+ addstate s1 (addstate s2 s3) = addstate (addstate s1 s2) s3.
+proof.
+rewrite /addstate; apply ext_eq => i Hi.
+by rewrite !map2iE // W64.WRing.AddMonoid.addmA. 
+qed.
+
+
+(**************************************************************
+    Functional Bit-oriented specification of KECCAK1600
+***************************************************************)
+
+lemma pad10star1P r m:
+ 0 < r =>
+ r %| size (m ++ pad10star1 r (size m)).
+proof.
+move=> Hr; rewrite dvdzE size_cat /pad10star1 /= size_rcons size_nseq.
+by rewrite ler_maxr 1:/# (addzC 1) /= -(addzC 2) addzA modzDmr /#.
+qed.
+
+lemma size_pad10star1 r len:
+ 0 < r =>
+ 0 <= len %% r <= r-2 =>
+ size (pad10star1 r len)
+ = r - (len %% r).
+proof.
+move=> Hr Hlen.
+rewrite /pad10star1 /= size_rcons size_nseq lez_maxr 1:/#.
+by rewrite -modzDml -modzNm -modzDl /#.
+qed.
+
+abbrev split_padded r m =
+ chunk r (m ++ pad10star1 r (size m)).
+
+op keccak1600_absorb_op (r: int, m: bits): state =
+ foldl
+  (fun s b => keccak_f1600_op (addstate s b))
+  st0
+  (map bits2state (split_padded r m)).
+
+(** Iterates [KECCAK_F1600] on [st] *)
+op st_i st i = iter i keccak_f1600_op st.
+
+op keccak1600_squeeze_op (r: int, st: state, outlen: int): bits =
+ take outlen 
+      (flatten
+        (List.map (take r \o state2bits \o st_i st)
+                  (iota_ 0 ((outlen-1) %/ r + 1)))).
+
+op keccak1600_sponge_op (r: int, m: bits, outlen: int): bits =
+ keccak1600_squeeze_op r (keccak1600_absorb_op r m) outlen.
+
+op keccak1600_op (c: int, m:bits, outlen: int): bits =
+ keccak1600_sponge_op (1600-c) m outlen.
+
+op SHA_DS_BITS = [false; true].
+op SHAKE_DS_BITS = [true; true; true; true].
+op RAWSHAKE_DS_BITS = [true; true].
+
+op sha3_224_op (m: bits): bits =
+ keccak1600_op 448 (m++SHA_DS_BITS) 224.
+op sha3_256_op (m: bits): bits =
+ keccak1600_op 512 (m++SHA_DS_BITS) 256.
+op sha3_384_op (m: bits): bits =
+ keccak1600_op 768 (m++SHA_DS_BITS) 384.
+op sha3_512_op (m: bits): bits =
+ keccak1600_op 1024 (m++SHA_DS_BITS) 512.
+op shake128_op (m: bits, outlen:int): bits =
+ keccak1600_op 256 (m++SHAKE_DS_BITS) outlen.
+op shake256_op (m: bits, outlen:int): bits =
+ keccak1600_op 512 (m++SHAKE_DS_BITS) outlen.
+op rawshake128_op (m: bits, outlen:int): bits =
+ keccak1600_op 256 (m++RAWSHAKE_DS_BITS) outlen.
+op rawshake256_op (m: bits, outlen:int): bits =
+ keccak1600_op 512 (m++RAWSHAKE_DS_BITS) outlen.
+
+(** A more convenient version of the sponge construction *)
+module SpongeBits = {
+  proc absorb(r: int, m: bits): state = {
+    var p, pl, n, s, i;
+    
+    p <- pad10star1 r (size m);
+    p <- m ++ p;
+    pl <- chunk r p;
+    n <- size p %/ r;
+    s <- st0;
+    i <- 0;
+    while (i < n){
+      s <- addstate s (bits2state (nth [] pl i));
+      s <- keccak_f1600_op(s);
+      i <- i + 1;
+    }
+    return s;
+  }
+  proc squeeze(r: int, s: state, d: int) = {
+    var z, i;
+    z <- take r (state2bits s);
+    i <- 1;
+    while (r*i < d){
+      s <- keccak_f1600_op(s);
+      z <- z ++ take r (state2bits s);
+      i <- i + 1;
+    }
+    
+    return take d z;
+  }
+  proc sponge(r:int, m: bits, d: int): bits = {
+    var s, o;
+    s <@ absorb(r, m);
+    o <@ squeeze(r, s, d);
+    return o;
+  }
+}.
+
+equiv keccak1600_sponge_eq:
+ Sponge1600(Keccakf1600_Params).sponge ~ SpongeBits.sponge
+ : ={r, m, d} /\ 0 <= r{2} <= 1600 ==> ={res}.
+proof.
+proc; inline absorb squeeze; simplify.
+wp; while (#pre /\ (z,s){1}=(z,s1){2} /\ (d0=d /\ r1=r /\ r*i0=size z){2}).
+ wp; ecall{1} (keccak_f1600_ph s{1}); auto => /> &1 &2 *.
+ by rewrite size_cat size_take' 1:/# !size_state2bits /#. 
+wp.
+while (#pre /\ (pl,n,i,s){1}=(pl,n,i,s0){2}).
+ by wp; ecall{1} (keccak_f1600_ph s{1}); auto => /> &1 &2 *.
+inline*; auto => /> &m *.
+by rewrite size_take' 1:/# size_state2bits /#.
+qed.
+
+phoare keccak1600_absorb_ll: 
+ [ SpongeBits.absorb
+ : 0 < r <= 1600 ==> true
+ ] = 1%r.
+proof.
+proc; wp; while (0<=i) (n-i).
+ by move=> z; auto => /> &m * /#.
+by auto => /> &m ??i /#.
+qed.
+
+phoare keccak1600_squeeze_ll: 
+ [ SpongeBits.squeeze
+ : 0 < r <= 1600 ==> true
+ ] = 1%r.
+proof.
+proc; wp; while (0<r /\ 0<=i) (d-r*i).
+ by move=> z; auto => /> &m * /#.
+by auto => /> &m ??i /#.
+qed.
+
+phoare keccak1600_sponge_ll: 
+ [ SpongeBits.sponge
+ : 0 < r <= 1600 ==> true
+ ] = 1%r.
+proof.
+proc; call keccak1600_squeeze_ll.
+by call keccak1600_absorb_ll.
+qed.
+
+phoare keccak1600_ll: 
+ [ Keccak1600.keccak1600
+ : 0 <= c < 1600 ==> true
+ ] = 1%r.
+proof.
+proc; simplify.
+call (: 0 < r && r <= 1600 ==> true).
+ conseq keccak1600_sponge_eq keccak1600_sponge_ll => /> &m *.
+ by exists (r{m},m{m},d{m}) => /> /#.
+by auto => /> /#.
+qed.
+
+hoare keccak1600_absorb_h _r _m:
+ SpongeBits.absorb
+ : r=_r /\ m=_m /\ 0<_r<=1600 ==> res = keccak1600_absorb_op _r _m.
+proof.
+proc; simplify.
+while (#pre /\ pl=split_padded r m /\ n=size pl /\ 0<=i<=n /\
+       keccak1600_absorb_op r m
+       = foldl (fun s b => keccak_f1600_op (addstate s b)) s (drop i (map bits2state pl))).
+ auto => /> &m ????H?; split; 1:smt().
+ rewrite H (foldl_dropS st0) /=.
+  by rewrite size_map /#.
+ congr; congr; congr.
+ by rewrite (nth_map []) 1:/#.
+auto => /> *; rewrite size_chunk 1:/#.
+split; 1:smt(drop0 size_ge0).
+move=> i s ?_?? ->; have ->: i=size (split_padded _r _m).
+ by rewrite size_chunk /#.
+by rewrite drop_oversize // size_map.
+qed.
+
+phoare keccak1600_absorb_ph _r _m:
+ [ SpongeBits.absorb
+ : r=_r /\ m=_m /\ 0<_r<=1600 ==> res = keccak1600_absorb_op _r _m
+ ] = 1%r.
+proof. by conseq keccak1600_absorb_ll (keccak1600_absorb_h _r _m). qed.
+
+hoare keccak1600_squeeze_h _r _s _d:
+ SpongeBits.squeeze
+ : r=_r /\ s=_s /\ d=_d /\ 0<_r<=1600
+ ==> res = keccak1600_squeeze_op _r _s _d.
+proof.
+proc; simplify.
+case: (d <= 0).
+ while (d=_d).
+  by auto => />.
+ by auto => /> *; rewrite /keccak1600_squeeze_op !take_le0 //.
+while (r=_r /\ d=_d /\ 0<_r<=1600 /\ 1<=i /\ r*i=size z /\ r*(i-1) < d /\
+       s = st_i _s (i-1) /\
+       z = flatten (map (take r \o state2bits \o st_i _s) (iota_ 0 i))).
+ auto => /> &m ???H??; rewrite !size_cat.
+ rewrite !size_take' 1:/#.
+ rewrite ifT.
+  rewrite size_state2bits /#.
+ split; 1:smt().
+ split; 1:smt().
+ split.
+  by rewrite {-1}(:i{m}=i{m}-1+1) 1:/# /st_i iterS 1:/# //.
+ rewrite iotaSr 1:/# map_rcons flatten_rcons; congr.
+ rewrite /(\o) /=; congr; congr.
+ by rewrite /st_i -iterS /#.
+auto => /> ???; split.
+ rewrite size_take' 1:/# size_state2bits ifT 1:/# /st_i iter0 1:/# => />.
+ by rewrite -iotaredE /(\o) /flatten /= iter0 1:/# cats0 /#.
+move=> i *; rewrite /keccak1600_sponge_op /keccak1600_squeeze_op.
+by congr; congr; congr; congr; smt().
+qed.
+
+phoare keccak1600_squeeze_ph _r _s _d:
+ [ SpongeBits.squeeze
+ : r=_r /\ s=_s /\ d=_d /\ 0<_r<=1600
+ ==> res = keccak1600_squeeze_op _r _s _d
+ ] = 1%r.
+proof. by conseq keccak1600_squeeze_ll (keccak1600_squeeze_h _r _s _d). qed.
+
+(** Standard spec. vs Functional spec. *)
+hoare keccak1600_h _c _m _outlen:
+ Keccak1600.keccak1600
+ : c = _c /\ m = _m /\ outlen = _outlen
+   /\ 0 <= _c < 1600
+ ==> res = keccak1600_sponge_op (1600-_c) _m _outlen.
+proof.
+bypr => /> &m' *.
+have ->: Pr[Keccak1600.keccak1600(c{m'}, m{m'}, outlen{m'}) @ &m' : res <> keccak1600_sponge_op (1600-c{m'}) m{m'} outlen{m'}] = Pr[SpongeBits.sponge(1600-c{m'}, m{m'}, outlen{m'}) @ &m' : res <> keccak1600_sponge_op (1600-c{m'}) m{m'} outlen{m'}]. 
+ byequiv => //.
+ proc*; inline keccak1600.
+ by wp; call keccak1600_sponge_eq; auto => /> /#.
+byphoare (: r=1600-c{m'} /\ m=m{m'} /\ d=outlen{m'} ==> _) => //; hoare; simplify.
+proc; inline sponge; simplify.
+ecall (keccak1600_squeeze_h r s d).
+ecall (keccak1600_absorb_h r m).
+by auto => /> /#.
+qed.
+
+phoare keccak1600_ph _c _m _outlen:
+ [ Keccak1600.keccak1600
+ : c = _c /\ m = _m /\ outlen = _outlen
+   /\ 0 < _c < 1600
+ ==> res = keccak1600_sponge_op (1600-_c) _m _outlen
+ ] = 1%r.
+proof.
+by conseq keccak1600_ll (keccak1600_h _c _m _outlen) => /> /#.
+qed.
+
+hoare sha3_224_h _m:
+ Keccak1600.sha3_224
+ : m = _m ==> res = sha3_224_op _m.
+proof.
+proc.
+by call (keccak1600_h 448 (_m ++ [false; true]) 224).
+qed.
+
+phoare sha3_224_ph _m:
+ [ Keccak1600.sha3_224
+ : m = _m ==> res = sha3_224_op _m
+ ] = 1%r.
+proof.
+have Hll: islossless Keccak1600.sha3_224 by proc; call keccak1600_ll.
+by conseq Hll (sha3_224_h _m).
+qed.
+
+hoare sha3_256_h _m:
+ Keccak1600.sha3_256
+ : m = _m ==> res = sha3_256_op _m.
+proof.
+proc.
+by call (keccak1600_h 512 (_m ++ [false; true]) 256).
+qed.
+
+phoare sha3_256_ph _m:
+ [ Keccak1600.sha3_256
+ : m = _m ==> res = sha3_256_op _m
+ ] = 1%r.
+proof.
+have Hll: islossless Keccak1600.sha3_256 by proc; call keccak1600_ll.
+by conseq Hll (sha3_256_h _m).
+qed.
+
+hoare sha3_384_h _m:
+ Keccak1600.sha3_384
+ : m = _m ==> res = sha3_384_op _m.
+proof.
+proc.
+by call (keccak1600_h 768 (_m ++ [false; true]) 384).
+qed.
+
+phoare sha3_384_ph _m:
+ [ Keccak1600.sha3_384
+ : m = _m ==> res = sha3_384_op _m
+ ] = 1%r.
+proof.
+have Hll: islossless Keccak1600.sha3_384 by proc; call keccak1600_ll.
+by conseq Hll (sha3_384_h _m).
+qed.
+
+hoare sha3_512_h _m:
+ Keccak1600.sha3_512
+ : m = _m ==> res = sha3_512_op _m.
+proof.
+proc.
+by call (keccak1600_h 1024 (_m ++ [false; true]) 512).
+qed.
+
+phoare sha3_512_ph _m:
+ [ Keccak1600.sha3_512
+ : m = _m ==> res = sha3_512_op _m
+ ] = 1%r.
+proof.
+have Hll: islossless Keccak1600.sha3_512 by proc; call keccak1600_ll.
+by conseq Hll (sha3_512_h _m).
+qed.
+
+hoare shake128_h _m _d:
+ Keccak1600.shake128
+ : m = _m /\ d = _d ==> res = shake128_op _m _d.
+proof.
+proc.
+by call (keccak1600_h 256 (_m ++ [true; true; true; true]) _d).
+qed.
+
+phoare shake128_ph _m _d:
+ [ Keccak1600.shake128
+ : m = _m /\ d = _d ==> res = shake128_op _m _d
+ ] = 1%r.
+proof.
+have Hll: islossless Keccak1600.shake128 by proc; call keccak1600_ll.
+by conseq Hll (shake128_h _m _d).
+qed.
+
+hoare shake256_h _m _d:
+ Keccak1600.shake256
+ : m = _m /\ d = _d ==> res = shake256_op _m _d.
+proof.
+proc.
+by call (keccak1600_h 512 (_m ++ [true; true; true; true]) _d).
+qed.
+
+phoare shake256_ph _m _d:
+ [ Keccak1600.shake256
+ : m = _m /\ d = _d ==> res = shake256_op _m _d
+ ] = 1%r.
+proof.
+have Hll: islossless Keccak1600.shake256 by proc; call keccak1600_ll.
+by conseq Hll (shake256_h _m _d).
+qed.
+
+hoare rawshake128_h _m _d:
+ Keccak1600.rawSHAKE128
+ : m = _m /\ d = _d ==> res = rawshake128_op _m _d.
+proof.
+proc.
+by call (keccak1600_h 256 (_m ++ [true; true]) _d).
+qed.
+
+phoare rawshake128_ph _m _d:
+ [ Keccak1600.rawSHAKE128
+ : m = _m /\ d = _d ==> res = rawshake128_op _m _d
+ ] = 1%r.
+proof.
+have Hll: islossless Keccak1600.rawSHAKE128 by proc; call keccak1600_ll.
+by conseq Hll (rawshake128_h _m _d).
+qed.
+
+hoare rawshake256_h _m _d:
+ Keccak1600.rawSHAKE256
+ : m = _m /\ d = _d ==> res = rawshake256_op _m _d.
+proof.
+proc.
+by call (keccak1600_h 512 (_m ++ [true; true]) _d).
+qed.
+
+phoare rawshake256_ph _m _d:
+ [ Keccak1600.rawSHAKE256
+ : m = _m /\ d = _d ==> res = rawshake256_op _m _d
+ ] = 1%r.
+proof.
+have Hll: islossless Keccak1600.rawSHAKE256 by proc; call keccak1600_ll.
+by conseq Hll (rawshake256_h _m _d).
+qed.
+
